WIP in instantiation theorem

pcuic/theories/PCUICInst.v
@@ -1,10 +1,9 @@
-
 (* Distributed under the terms of the MIT license. *)
 From Coq Require Import Morphisms.
 From MetaCoq.Template Require Import config utils.
 From MetaCoq.PCUIC Require Import PCUICAst PCUICAstUtils PCUICCases PCUICInduction
   PCUICLiftSubst PCUICUnivSubst PCUICTyping PCUICClosed PCUICEquality PCUICWeakeningEnv
-  PCUICRename.
+  PCUICSigmaCalculus PCUICRename PCUICWeakening.
 
 Require Import ssreflect ssrbool.
 From Equations Require Import Equations.
@@ -13,13 +12,22 @@ Set Equations With UIP.
 Set Keyed Unification.
 Set Default Goal Selector "!".
 
+Implicit Types cf : checker_flags.
+
 (** * Type preservation for σ-calculus instantiation *)
 
 Open Scope sigma_scope.
 
 Definition inst_context σ (Γ : context) : context :=
   fold_context (fun i => inst (⇑^i σ)) Γ.
-  
+
+Instance inst_context_ext : Proper (`=1` ==> Logic.eq ==> Logic.eq) inst_context.
+Proof.
+  intros f g Hfg x y ->.
+  apply fold_context_ext => i t.
+  now rewrite Hfg.
+Qed.
+
 Definition inst_decl σ d := map_decl (inst σ) d.
 
 Definition inst_context_snoc0 s Γ d :
@@ -56,19 +64,15 @@ Lemma lift0_inst n t : lift0 n t = t.[↑^n].
 Proof. by rewrite lift_rename rename_inst lift_renaming_0 -ren_shiftk. Qed.
 Hint Rewrite lift0_inst : sigma.
 
-Lemma rename_decl_inst_decl :
-  forall f d,
-    rename_decl f d = inst_decl (ren f) d.
+Lemma rename_decl_inst_decl : forall f d, rename_decl f d = inst_decl (ren f) d.
 Proof.
   intros f d.
   unfold rename_decl, inst_decl.
   destruct d. unfold map_decl.
   autorewrite with sigma.
   f_equal.
-  simpl. destruct decl_body.
-  - simpl. f_equal. autorewrite with sigma. reflexivity.
-  - reflexivity.
 Qed.
+
 Hint Rewrite rename_decl_inst_decl : sigma.
 
 Lemma rename_context_inst_context :
@@ -219,7 +223,7 @@ Proof.
   now rewrite [map_decl _ _]inst_decl_closed.
 Qed.
 
-Lemma typed_inst :
+Lemma typed_inst {cf} :
   forall Σ Γ t T k σ,
     wf Σ.1 ->
     k >= #|Γ| ->
@@ -238,7 +242,7 @@ Proof.
   rewrite !inst_closed. all: auto.
 Qed.
 
-Lemma inst_wf_local :
+Lemma inst_wf_local {cf} :
   forall Σ Γ σ,
     wf Σ.1 ->
     wf_local Σ Γ ->
@@ -261,78 +265,6 @@ Qed.
 Definition inst_mutual_inductive_body σ m :=
   map_mutual_inductive_body (fun i => inst (⇑^i σ)) m.
 
-Lemma inst_declared_minductive :
-  forall Σ cst decl σ,
-    wf Σ ->
-    declared_minductive Σ cst decl ->
-    inst_mutual_inductive_body σ decl = decl.
-Proof.
-Admitted.
-(*
-  unfold declared_minductive.
-  intros Σ cst decl σ hΣ h.
-  eapply lookup_on_global_env in h ; eauto. simpl in h.
-  destruct h as [Σ' [hΣ' decl']].
-  destruct decl as [fi npars params bodies univs]. simpl. f_equal.
-  - eapply inst_wf_local. all: eauto.
-    eapply onParams in decl'. auto.
-  - apply onInductives in decl'.
-    revert decl'. generalize bodies at 2 4 5. intros bodies' decl'.
-    eapply Alli_mapi_id in decl'. all: eauto.
-    clear decl'. intros n [na ty ke ct pr] hb. simpl.
-    destruct (decompose_prod_assum [] ty) as [c t] eqn:e1.
-    destruct (decompose_prod_assum [] ty.[⇑^0 σ]) as [c' t'] eqn:e2.
-    destruct hb as [indices s arity_eq onAr csorts onConstr onProj sorts].
-    simpl in *.
-    assert (e : ty.[⇑^0 σ] = ty).
-    { destruct onAr as [s' h'].
-      eapply typed_inst in h' as [_ ?]. all: eauto.
-    }
-    rewrite e in e2. rewrite e1 in e2.
-    revert e2. intros [= <- <-].
-    rewrite e. f_equal.
-    + eapply All_map_id. eapply All2_All_left; tea.
-      intros [[x p] n'] y [[?s Hty] [cs Hargs]].
-      unfold on_pi2; cbn; f_equal; f_equal.
-      eapply typed_inst. all: eauto.
-    + destruct (eq_dec pr []) as [hp | hp]. all: subst. all: auto.
-      specialize (onProj hp).
-      apply on_projs in onProj.
-      apply (Alli_map_id onProj).
-      intros n1 [x p]. unfold on_projection. simpl.
-      intros [? hty].
-      unfold on_snd. simpl. f_equal.
-      eapply typed_inst. all: eauto.
-      simpl.
-      rewrite smash_context_length context_assumptions_fold.
-      simpl. auto.
-Qed.*)
-
-Lemma inst_declared_inductive :
-  forall Σ ind mdecl idecl σ,
-    wf Σ ->
-    declared_inductive Σ ind mdecl idecl ->
-    map_one_inductive_body
-      (context_assumptions mdecl.(ind_params))
-      #|arities_context mdecl.(ind_bodies)|
-      (fun i => inst (⇑^i σ))
-      ind.(inductive_ind)
-      idecl
-    = idecl.
-Proof.
-  intros Σ ind mdecl idecl σ hΣ [hmdecl hidecl].
-  eapply inst_declared_minductive with (σ := σ) in hmdecl. all: auto.
-  unfold inst_mutual_inductive_body in hmdecl.
-  destruct mdecl as [fi npars params bodies univs]. simpl in *.
-  injection hmdecl. intro e. clear hmdecl.
-  pose proof hidecl as hidecl'.
-  rewrite <- e in hidecl'.
-  rewrite nth_error_mapi in hidecl'.
-  clear e.
-  unfold option_map in hidecl'. rewrite hidecl in hidecl'.
-  congruence.
-Qed.
-
 Lemma inst_destArity :
   forall ctx t σ args s,
     destArity ctx t = Some (args, s) ->
@@ -349,150 +281,61 @@ Proof.
     simpl. autorewrite with sigma. reflexivity.
 Qed.
 
+Lemma Up_subst_instance_constr u σ :
+  ⇑ (subst_instance_constr u ∘ σ) =1 subst_instance_constr u ∘ ⇑ σ.
+Proof.
+  intros i => /=.
+  rewrite - !up_Up /up.
+  nat_compare_specs => //.
+  now rewrite rename_subst_instance_constr.
+Qed.
 
-(* Lemma types_of_case_rename : *)
-(*   forall Σ ind mdecl idecl npar args u p pty indctx pctx ps btys f, *)
-(*     wf Σ -> *)
-(*     declared_inductive Σ ind mdecl idecl -> *)
-(*     types_of_case ind mdecl idecl (firstn npar args) u p pty = *)
-(*     Some (indctx, pctx, ps, btys) -> *)
-(*     types_of_case *)
-(*       ind mdecl idecl *)
-(*       (firstn npar (map (rename f) args)) u (rename f p) (rename f pty) *)
-(*     = *)
-(*     Some ( *)
-(*         rename_context f indctx, *)
-(*         rename_context f pctx, *)
-(*         ps, *)
-(*         map (on_snd (rename f)) btys *)
-(*     ). *)
-(* Proof. *)
-(*   intros Σ ind mdecl idecl npar args u p pty indctx pctx ps btys f hΣ hdecl h. *)
-(*   unfold types_of_case in *. *)
-(*   case_eq (instantiate_params (subst_instance_context u (ind_params mdecl)) (firstn npar args) (subst_instance_constr u (ind_type idecl))) ; *)
-(*     try solve [ intro bot ; rewrite bot in h ; discriminate h ]. *)
-(*   intros ity eity. rewrite eity in h. *)
-(*   pose proof (on_declared_inductive hΣ as hdecl) [onmind onind]. *)
-(*   apply onParams in onmind as Hparams. *)
-(*   assert (closedparams : closed_ctx (subst_instance_context u (ind_params mdecl))). *)
-(*   { rewrite closedn_subst_instance_context. *)
-(*     eapply PCUICWeakening.closed_wf_local. all: eauto. eauto. } *)
-(*   epose proof (inst_declared_inductive _ mdecl ind idecl (ren f) hΣ) as hi. *)
-(*   forward hi by assumption. rewrite <- hi. *)
-(*   eapply instantiate_params_rename with (f := f) in eity ; auto. *)
-(*   rewrite -> ind_type_map. *)
-(*   rewrite firstn_map. *)
-(*   lazymatch type of eity with *)
-(*   | ?t = _ => *)
-(*     lazymatch goal with *)
-(*     | |- match ?t' with _ => _ end = _ => *)
-(*       replace t' with t ; revgoals *)
-(*     end *)
-(*   end. *)
-(*   { autorewrite with sigma. *)
-(*     rewrite <- !rename_inst. *)
-(*     now rewrite rename_subst_instance_constr. } *)
-(*   rewrite eity. *)
-(*   case_eq (destArity [] ity) ; *)
-(*     try solve [ intro bot ; rewrite bot in h ; discriminate h ]. *)
-(*   intros [args0 ?] ear. rewrite ear in h. *)
-(*   eapply inst_destArity with (σ := ren f) in ear as ear'. *)
-(*   simpl in ear'. *)
-(*   lazymatch type of ear' with *)
-(*   | ?t = _ => *)
-(*     lazymatch goal with *)
-(*     | |- match ?t' with _ => _ end = _ => *)
-(*       replace t' with t ; revgoals *)
-(*     end *)
-(*   end. *)
-(*   { autorewrite with sigma. reflexivity. } *)
-(*   rewrite ear'. *)
-(*   case_eq (destArity [] pty) ; *)
-(*     try solve [ intro bot ; rewrite bot in h ; discriminate h ]. *)
-(*   intros [args' s'] epty. rewrite epty in h. *)
-(*   eapply inst_destArity with (σ := ren f) in epty as epty'. *)
-(*   simpl in epty'. *)
-(*   lazymatch type of epty' with *)
-(*   | ?t = _ => *)
-(*     lazymatch goal with *)
-(*     | |- match ?t' with _ => _ end = _ => *)
-(*       replace t' with t ; revgoals *)
-(*     end *)
-(*   end. *)
-(*   { autorewrite with sigma. reflexivity. } *)
-(*   rewrite epty'. *)
-(*   case_eq (map_option_out (build_branches_type ind mdecl idecl (firstn npar args) u p)) ; *)
-(*     try solve [ intro bot ; rewrite bot in h ; discriminate h ]. *)
-(*   intros brtys ebrtys. rewrite ebrtys in h. *)
-(*   inversion h. subst. clear h. *)
-(*   eapply build_branches_type_rename with (f := f) in ebrtys as ebrtys'. *)
-(*   2: assumption. *)
-(*   lazymatch type of ebrtys' with *)
-(*   | ?t = _ => *)
-(*     lazymatch goal with *)
-(*     | |- match ?t' with _ => _ end = _ => *)
-(*       replace t' with t ; revgoals *)
-(*     end *)
-(*   end. *)
-(*   { f_equal. f_equal. unfold map_one_inductive_body. destruct idecl. *)
-(*     simpl. f_equal. *)
-(*     - autorewrite with sigma. *)
-(*       eapply inst_ext. intro j. *)
-(*       unfold ren, shiftn. simpl. *)
-(*       f_equal. f_equal. lia. *)
-(*     - clear. induction ind_ctors. 1: reflexivity. *)
-(*       simpl. unfold on_pi2. destruct a. simpl. *)
-(*       destruct p. simpl. f_equal. 2: easy. *)
-(*       f_equal. f_equal. *)
-(*       autorewrite with sigma. *)
-(*       eapply inst_ext. intro j. *)
-(*       unfold ren, Upn, shiftn, subst_consn. *)
-(*       rewrite arities_context_length. *)
-(*       destruct (Nat.ltb_spec j #|ind_bodies mdecl|). *)
-(*       + rewrite nth_error_idsn_Some. all: easy. *)
-(*       + rewrite nth_error_idsn_None. 1: auto. *)
-(*         unfold subst_compose, shiftk. simpl. *)
-(*         rewrite idsn_length. reflexivity. *)
-(*     - clear. induction ind_projs. 1: auto. *)
-(*       simpl. destruct a. unfold on_snd. simpl. *)
-(*       f_equal. 2: easy. *)
-(*       f_equal. autorewrite with sigma. *)
-(*       eapply inst_ext. intro j. *)
-(*       unfold Upn, Up, ren, shiftn, subst_cons, subst_consn, subst_compose, *)
-(*       shift, shiftk. *)
-(*       destruct j. *)
-(*       + simpl. reflexivity. *)
-(*       + simpl. *)
-(*         destruct (Nat.ltb_spec (S j) (S (context_assumptions (ind_params mdecl)))). *)
-(*         * rewrite nth_error_idsn_Some. 1: lia. *)
-(*           simpl. reflexivity. *)
-(*         * rewrite nth_error_idsn_None. 1: lia. *)
-(*           simpl. rewrite idsn_length. reflexivity. *)
-(*   } *)
-(*   rewrite ebrtys'. autorewrite with sigma. reflexivity. *)
-(* Qed. *)
+Lemma upn_subst_instance_constr u n σ :
+  up n (subst_instance_constr u ∘ σ) =1 subst_instance_constr u ∘ up n σ.
+Proof.
+  intros i => /=.
+  rewrite /up.
+  nat_compare_specs => //.
+  now rewrite rename_subst_instance_constr.
+Qed.
 
+Lemma Upn_subst_instance_constr u n σ :
+  ⇑^n (subst_instance_constr u ∘ σ) =1 subst_instance_constr u ∘ ⇑^n σ.
+Proof.
+  rewrite - !up_Upn. rewrite upn_subst_instance_constr.
+  intros i. now rewrite up_Upn.
+Qed.
 
 Lemma inst_subst_instance_constr :
   forall u t σ,
-    (subst_instance_constr u t).[(subst_instance_constr u ∘ σ)%prog] =
+    (subst_instance_constr u t).[subst_instance_constr u ∘ σ] =
     subst_instance_constr u t.[σ].
 Proof.
   intros u t σ.
   induction t in σ |- * using term_forall_list_ind.
+  all: try solve [
+    simpl ;
+    rewrite ?IHt ?IHt1 ?IHt2 ;
+    easy
+  ].
   all: simpl. all: auto.
-  all: autorewrite with sigma.
-  all: rewrite ?map_map_compose ?compose_on_snd ?compose_map_def ?map_lenght.
+  all: rewrite ?map_map_compose ?compose_on_snd ?compose_map_def ?map_length
+    ?map_predicate_map_predicate ?map_branch_map_branch.
   all: try solve [ f_equal ; eauto ; solve_all ; eauto ].
-  - rewrite IHt1. f_equal. rewrite <- IHt2.
-    eapply inst_ext. intro i.
-    unfold Up, subst_compose, subst_cons.
-    destruct i.
-    + reflexivity.
-    + pose proof (shift_subst_instance_constr u (σ i) 0) as e.
-      autorewrite with sigma in e. rewrite e. reflexivity.
-  -  f_equal;auto.
-Admitted.
+  all: try now rewrite IHt1; sigma; rewrite-IHt2 -?IHt3 ?Up_subst_instance_constr.
+  - f_equal; auto.
+    * solve_all. 
+      now rewrite upn_subst_instance_constr e.
+    * solve_all. rewrite !map_branch_map_branch; solve_all.
+      apply map_branch_eq_spec.
+      now rewrite upn_subst_instance_constr H.
+  - f_equal. solve_all.
+    apply map_def_eq_spec; auto.
+    now rewrite upn_subst_instance_constr.
+  - f_equal; solve_all.
+    apply map_def_eq_spec; auto.
+    now rewrite upn_subst_instance_constr.
+Qed.
 
 Lemma map_vass_map_def_inst g l s :
   (mapi (fun i (d : def term) => vass (dname d) (lift0 i (dtype d)))
@@ -531,43 +374,70 @@ Definition well_subst Σ (Γ : context) σ (Δ : context) :=
     Σ ;;; Δ |- σ x : ((lift0 (S x)) (decl_type decl)).[ σ ] ×
     (forall b,
         decl.(decl_body) = Some b ->
-        σ x = b.[⇑^(S x) σ]
-    ).
+        (∑ x' decl', σ x = tRel x' ×
+          nth_error Δ x' = Some decl' ×
+          (* Γ_x', x := b : ty -> Δ_x', x' := b.[↑^S x ∘s σ]. 
+             Δ |- ↑^(S x) ∘s σ : Γ_x
+            *)
+          option_map (rename (rshiftk (S x'))) decl'.(decl_body) = Some (b.[↑^(S x) ∘s σ])) +
+        (σ x = b.[↑^(S x) ∘s ⇑ σ])).
 
 Notation "Σ ;;; Δ ⊢ σ : Γ" :=
   (well_subst Σ Γ σ Δ) (at level 50, Δ, σ, Γ at next level).
-
-Lemma well_subst_Up :
-  forall Σ Γ Δ σ na A,
-    wf_local Σ (Δ ,, vass na A.[σ]) ->
-    Σ ;;; Δ ⊢ σ : Γ ->
-    Σ ;;; Δ ,, vass na A.[σ] ⊢ ⇑ σ : Γ ,, vass na A.
+(* 
+Lemma shift_Up_comm σ : ↑ ∘s ⇑ σ =1 ⇑ (⇑ σ).
 Proof.
-  intros Σ Γ Δ σ na A hΔ h [|n] decl e.
+  intros i. unfold subst_compose. simpl.
+  unfold subst_compose, Up. simpl.
+  destruct i.
+  sigma. *)
+Lemma well_subst_Up {Σ : global_env_ext} {wfΣ : wf Σ} {Γ Δ σ na A} :
+  wf_local Σ (Δ ,, vass na A.[σ]) ->
+  Σ ;;; Δ ⊢ σ : Γ ->
+  Σ ;;; Δ ,, vass na A.[σ] ⊢ ⇑ σ : Γ ,, vass na A.
+Proof.
+  intros hΔ h [|n] decl e.
   - simpl in *. inversion e. subst. clear e. simpl.
     split.
     + eapply meta_conv.
       * econstructor ; auto.
         reflexivity.
       * simpl.
-        autorewrite with sigma.
-        eapply inst_ext. intro i.
-        unfold subst_compose.
-        eapply inst_ext. intro j.
-        unfold shift, ren. reflexivity.
+        now autorewrite with sigma.
     + intros b e. discriminate.
-  - simpl in *.
+  - cbn -[rshiftk] in *.
     specialize (h _ _ e) as [h1 h2].
     split.
-Admitted.
+    + sigma. sigma in h1.
+      eapply meta_conv.
+      * epose proof (weakening_rename_typing (Γ' := []) (Γ'' := [_]) hΔ h1).
+        simpl in X.
+        sigma in X. eapply X.
+      * eapply inst_ext. rewrite ren_lift_renaming.
+        now sigma.
+    + intros b hb.
+      specialize (h2 _ hb) as [[x' [decl' [hrel [hnth hdecl]]]]|].
+      * left. exists (S x'), decl'.
+        split.
+        ** unfold subst_compose at 1. now rewrite hrel.
+        ** cbn -[rshiftk]. split; auto.
+           destruct (decl_body decl') => //. cbn -[rshiftk] in hdecl |- *.
+           noconf hdecl. f_equal.
+           replace (S (S n)) with (S n + 1) by lia.
+           rewrite -shiftk_compose subst_compose_assoc.
+           rewrite -Upn_1_Up (shiftn_consn_idsn 1) -subst_compose_assoc -inst_assoc -H0.
+           sigma. now rewrite ren_shift compose_ren.
+      * right.
+        unfold subst_compose at 1. rewrite e0.
+        now rewrite inst_assoc.
+Qed.
 
-Lemma well_subst_Up' :
-  forall Σ Γ Δ σ na t A,
-    wf_local Σ (Δ ,, vdef na t.[σ] A.[σ]) ->
-    Σ ;;; Δ ⊢ σ : Γ ->
-    Σ ;;; Δ ,, vdef na t.[σ] A.[σ] ⊢ ⇑ σ : Γ ,, vdef na t A.
+Lemma well_subst_Up' {Σ : global_env_ext} {wfΣ : wf Σ} {Γ Δ σ na t A} :
+  wf_local Σ (Δ ,, vdef na t.[σ] A.[σ]) ->
+  Σ ;;; Δ ⊢ σ : Γ ->
+  Σ ;;; Δ ,, vdef na t.[σ] A.[σ] ⊢ ⇑ σ : Γ ,, vdef na t A.
 Proof.
-  intros Σ Γ Δ σ na t A wf h [|n] decl e.
+  intros wf h [|n] decl e.
   - simpl in *. inversion e. subst. clear e. simpl.
     rewrite lift_rename. rewrite rename_inst.
     autorewrite with sigma.
@@ -577,43 +447,525 @@ Proof.
       * rewrite lift0_inst /=.
         now autorewrite with sigma.
     + intros b [= ->].
-      (* well-subst is ill-definied it should allow  let-preservation *)
-      admit.
+      left. exists 0. eexists _; intuition eauto.
+      simpl. sigma. reflexivity.
+  - cbn -[rshiftk] in *.
+    specialize (h _ _ e) as [h1 h2].
+    split.
+    + sigma. sigma in h1.
+      eapply meta_conv.
+      * epose proof (weakening_rename_typing (Γ' := []) (Γ'' := [_]) wf h1).
+        simpl in X.
+        sigma in X. eapply X.
+      * eapply inst_ext. rewrite ren_lift_renaming.
+        now sigma.
+    + intros b hb.
+      specialize (h2 _ hb) as [[x' [decl' [hrel [hnth hdecl]]]]|].
+      * left. exists (S x'), decl'.
+        split.
+        ** unfold subst_compose at 1. now rewrite hrel.
+        ** cbn -[rshiftk]. split; auto.
+          destruct (decl_body decl') => //. cbn -[rshiftk] in hdecl |- *.
+          noconf hdecl. f_equal.
+          replace (S (S n)) with (S n + 1) by lia.
+          rewrite -shiftk_compose subst_compose_assoc.
+          rewrite -Upn_1_Up (shiftn_consn_idsn 1) -subst_compose_assoc -inst_assoc -H0.
+          sigma. now rewrite ren_shift compose_ren.
+      * right.
+        unfold subst_compose at 1. rewrite e0.
+        now rewrite inst_assoc.
+Qed.
 
-  - simpl in *.
-    specialize (h _ _ e).
-Admitted.
+Lemma well_subst_ext Σ Δ σ σ' Γ : 
+  Σ ;;; Δ ⊢ σ : Γ ->
+  σ =1 σ' ->
+  Σ ;;; Δ ⊢ σ' : Γ.
+Proof.
+  intros Hσ eq n decl hnth.
+  specialize (Hσ n decl hnth) as [hσ hb].
+  split.
+  - rewrite -(eq n).
+    eapply meta_conv. 2:now rewrite -eq. assumption.
+  - intros b hd. specialize (hb b hd).
+    destruct hb as [[x' [decl' [eqn [hnth' hsome]]]]|h].
+    * left; exists x', decl'. rewrite -(eq n). repeat split; auto.
+      now rewrite -eq.
+    * right. now rewrite -(eq n) -eq.
+Qed.
 
-(* (* Could be more precise *) *)
-(* Lemma instantiate_params_subst_length : *)
-(*   forall params pars s t s' t', *)
-(*     instantiate_params_subst params pars s t = Some (s', t') -> *)
-(*     #|params| >= #|pars|. *)
-(* Proof. *)
-(*   intros params pars s t s' t' h. *)
-(*   induction params in pars, s, t, s', t', h |- *. *)
-(*   - cbn in h. destruct pars. all: try discriminate. auto. *)
-(*   - cbn in h. destruct (decl_body a). *)
-(*     + destruct t. all: try discriminate. *)
-(*       cbn. eapply IHparams in h. lia. *)
-(*     + destruct t. all: try discriminate. *)
-(*       destruct pars. 1: discriminate. *)
-(*       cbn. eapply IHparams in h. lia. *)
-(* Qed. *)
+Lemma well_subst_app {Σ : global_env_ext} {wfΣ : wf Σ} {Γ Δ σ Δ'} :
+  wf_local Σ (Δ ,,, inst_context σ Δ') ->
+  Σ ;;; Δ ⊢ σ : Γ ->
+  Σ ;;; Δ ,,, inst_context σ Δ' ⊢ ⇑^#|Δ'| σ : Γ ,,, Δ'.
+Proof.
+  induction Δ' as [|[na [b|] ty] Δ']; simpl => hwf hsub.
+  - eapply well_subst_ext; eauto.
+    now rewrite Upn_0.
+  - rewrite inst_context_snoc.
+    eapply well_subst_ext.
+    2:now rewrite Upn_S. simpl.
+    apply well_subst_Up'.
+    * rewrite inst_context_snoc in hwf.
+      apply hwf.
+    * rewrite inst_context_snoc in hwf.
+      depelim hwf. apply IHΔ' => //.
+  - rewrite inst_context_snoc.
+    eapply well_subst_ext.
+    2:now rewrite Upn_S. simpl.
+    apply well_subst_Up.
+    * rewrite inst_context_snoc in hwf.
+      apply hwf.
+    * rewrite inst_context_snoc in hwf.
+      depelim hwf. apply IHΔ' => //.
+Qed.
 
-(* Lemma instantiate_params_length : *)
-(*   forall params pars T T', *)
-(*     instantiate_params params pars T = Some T' -> *)
-(*     #|params| >= #|pars|. *)
-(* Proof. *)
-(*   intros params pars T T' e. *)
-(*   unfold instantiate_params in e. *)
-(*   case_eq (instantiate_params_subst (List.rev params) pars [] T) ; *)
-(*     try solve [ intro bot ; rewrite bot in e ; discriminate e ]. *)
-(*   intros [s' t'] e'. rewrite e' in e. inversion e. subst. clear e. *)
-(*   eapply instantiate_params_subst_length in e'. *)
-(*   rewrite List.rev_length in e'. assumption. *)
-(* Qed. *)
+Lemma well_subst_app_up {Σ : global_env_ext} {wfΣ : wf Σ} {Γ Δ σ Δ'} :
+  wf_local Σ (Δ ,,, inst_context σ Δ') ->
+  Σ ;;; Δ ⊢ σ : Γ ->
+  Σ ;;; Δ ,,, inst_context σ Δ' ⊢ up #|Δ'| σ : Γ ,,, Δ'.
+Proof.
+  intros wf Hσ.
+  eapply well_subst_ext.
+  2:now rewrite up_Upn.
+  now apply well_subst_app.
+Qed.
+
+Notation inst_predicate f p :=
+  (map_predicate id (inst f) (inst (up #|pcontext p| f)) p).
+
+Lemma inst_predicate_preturn f p :
+  inst (⇑^#|p.(pcontext)| f) (preturn p) =
+  preturn (inst_predicate f p).
+Proof. rewrite -up_Upn. reflexivity. Qed.
+
+Lemma inst_mkLambda_or_LetIn f d t : 
+  inst f (mkLambda_or_LetIn d t) =
+  mkLambda_or_LetIn (inst_decl f d) (inst (⇑ f) t).
+Proof.
+  destruct d as [na [] ty]; rewrite /= /mkLambda_or_LetIn /=; f_equal; now rewrite up_Up.
+Qed.
+
+Lemma inst_it_mkLambda_or_LetIn f ctx t : 
+  inst f (it_mkLambda_or_LetIn ctx t) =
+  it_mkLambda_or_LetIn (inst_context f ctx) (inst (⇑^#|ctx| f) t).
+Proof.
+  move: t.
+  induction ctx; simpl => t.
+  - now rewrite Upn_0.
+  - rewrite /= IHctx inst_context_snoc /snoc /=. f_equal.
+    now rewrite inst_mkLambda_or_LetIn /=; sigma.
+Qed.
+
+Lemma inst_reln f ctx n acc :
+  forallb (closedn (n + #|ctx|)) acc ->
+  map (inst (⇑^(n + #|ctx|) f)) (reln acc n ctx) = 
+  reln acc n ctx.
+Proof.
+  induction ctx in n, acc |- *; simpl; auto.
+  - intros clacc. solve_all. 
+    now rewrite inst_closed.
+  - intros clacc.
+    destruct a as [? [] ?].
+    * rewrite Nat.add_succ_r.
+      change (S (n + #|ctx|)) with (S n + #|ctx|).
+      rewrite Nat.add_1_r IHctx // /= -Nat.add_succ_r //.
+    * rewrite Nat.add_succ_r Nat.add_1_r. rewrite (IHctx (S n)) /= // -Nat.add_succ_r //.
+      simpl. rewrite clacc andb_true_r.
+      eapply Nat.ltb_lt. lia.
+Qed.
+
+Lemma inst_to_extended_list f ctx :
+  map (inst (⇑^#|ctx| f)) (to_extended_list ctx) = to_extended_list ctx.
+Proof.
+  unfold to_extended_list, to_extended_list_k.
+  now apply (inst_reln _ _ 0).
+Qed.
+
+Lemma inst_subst :
+  forall f s n t,
+    inst (⇑^n f) (subst s n t) =
+    subst (map (inst f) s) n (inst (⇑^n (⇑^#|s| f)) t).
+Proof.
+  intros f s n t.
+  autorewrite with sigma.
+  eapply inst_ext. intro i. unfold Upn.
+  unfold subst_consn, shiftk, subst_compose. simpl.
+  destruct (Nat.ltb_spec i n).
+  - rewrite idsn_lt //. simpl.
+    rewrite idsn_lt //.
+  - rewrite nth_error_idsn_None //. len.
+    rewrite !inst_assoc. unfold subst_compose. simpl.
+    destruct (Nat.ltb_spec (i - n) #|s|).
+    * rewrite idsn_lt //. simpl.
+      rewrite nth_error_idsn_None //; try lia.
+      rewrite nth_error_map.
+      replace (n + (i - n) - n) with (i - n) by lia.
+      destruct nth_error eqn:hnth => /=.
+      ** sigma. apply inst_ext.
+        intros k. cbn.
+        elim: (Nat.ltb_spec (n + k) n); try lia.
+        intros. eapply nth_error_Some_length in hnth.
+        rewrite nth_error_idsn_None //. unfold subst_compose.
+        lia_f_equal.
+      ** eapply nth_error_None in hnth. lia.
+    * len.
+      rewrite nth_error_idsn_None; try lia.
+      rewrite inst_assoc. simpl.
+      destruct nth_error eqn:hnth.
+      ** eapply nth_error_Some_length in hnth. lia.
+      ** simpl.
+        eapply nth_error_None in hnth.
+        rewrite nth_error_idsn_None; try lia.
+        unfold subst_compose. simpl.
+        assert (n + (i - n - #|s|) - n = (i - n - #|s|)) as -> by lia.
+        apply inst_ext => k.
+        rewrite nth_error_idsn_None //; try lia.
+        destruct nth_error eqn:hnth'.
+        + eapply nth_error_Some_length in hnth'. len in hnth'. lia.
+        + simpl. lia_f_equal.
+Qed.
+
+Lemma inst_context_subst_k f s k Γ : 
+  inst_context (up k f) (subst_context s k Γ) =
+  subst_context (map (inst f) s) k (inst_context (⇑^(k + #|s|) f) Γ).
+Proof.
+  rewrite !inst_context_alt !subst_context_alt.
+  rewrite !mapi_mapi. apply mapi_ext => i x.
+  rewrite /subst_decl !compose_map_decl.
+  apply map_decl_ext => t.
+  len.
+  generalize (Nat.pred #|Γ| - i).
+  intros. rewrite up_Upn -Upn_Upn inst_subst.
+  now sigma.
+Qed.
+
+Lemma inst_context_subst f s Γ : 
+  inst_context f (subst_context s 0 Γ) =
+  subst_context (map (inst f) s) 0 (inst_context (⇑^#|s| f) Γ).
+Proof.
+  now rewrite -inst_context_subst_k up_Upn Upn_0.
+Qed.
+
+Lemma inst_case_predicate_context {Σ} {wfΣ : wf Σ} {ind mdecl idecl f p} :
+  declared_inductive Σ ind mdecl idecl ->
+  wf_predicate mdecl idecl p ->
+  inst_context f (case_predicate_context ind mdecl idecl p) =
+  case_predicate_context ind mdecl idecl (inst_predicate f p).
+Proof.
+  intros decli wfp.
+  unfold case_predicate_context. simpl.
+  unfold id. unfold case_predicate_context_gen.
+  rewrite /inst_context.
+  rewrite -map2_set_binder_name_fold //.
+  - len. len. 
+    now rewrite -(wf_predicate_length_pcontext wfp).
+  - f_equal. rewrite fold_context_snoc0 /= /snoc.
+    f_equal.
+    * rewrite /map_decl /=. f_equal.
+      len. rewrite inst_mkApps /=. f_equal.
+      rewrite !map_app !map_map_compose. f_equal.
+      + solve_all.
+        eapply All_refl => x.
+        sigma. now rewrite shiftn_consn_idsn.
+      + now rewrite inst_to_extended_list.
+    * rewrite -/(inst_context f _).
+      rewrite inst_context_subst.
+      f_equal.
+      rewrite inst_closedn_ctx //.
+      pose proof (closedn_ctx_expand_lets (ind_params mdecl) (ind_indices idecl)
+        (declared_inductive_closed_pars_indices _ decli)).
+      rewrite (wf_predicate_length_pars wfp).
+      rewrite (declared_minductive_ind_npars decli).
+      now rewrite closedn_subst_instance_context.
+Qed.
+
+Lemma inst_wf_predicate mdecl idecl f p :
+  wf_predicate mdecl idecl p ->
+  wf_predicate mdecl idecl (inst_predicate f p).
+Proof.
+  intros []. split.
+  - now len.
+  - assumption.
+Qed.
+
+Lemma inst_wf_branch cdecl f br :
+  wf_branch cdecl br ->
+  wf_branch cdecl (map_branch (inst (up #|br.(bcontext)| f)) br).
+Proof.
+  unfold wf_branch, wf_branch_gen. now simpl.
+Qed.
+
+Lemma inst_wf_branches cdecl f brs :
+  wf_branches cdecl brs ->
+  wf_branches cdecl (map (fun br => map_branch (inst (up #|br.(bcontext)| f)) br) brs).
+Proof.
+  unfold wf_branches, wf_branches_gen.
+  intros h. solve_all. eapply Forall2_map_right.
+  solve_all.
+Qed.
+ 
+Lemma wf_local_app_inst (Σ : global_env_ext) {wfΣ : wf Σ} Γ Δ : 
+  All_local_env (lift_typing (fun (Σ : global_env_ext) (Γ' : context) (t T : term) =>
+    forall Δ σ,
+    wf_local Σ Δ ->
+    Σ ;;; Δ ⊢ σ : (Γ ,,, Γ') ->
+    Σ ;;; Δ |- t.[σ] : T.[σ]) Σ) Δ ->
+  forall Δ' σ,
+  Σ ;;; Δ' ⊢ σ : Γ ->
+  wf_local Σ Δ' ->
+  wf_local Σ (Δ' ,,, inst_context σ Δ).
+Proof.
+  intros.
+  induction X.
+  - now simpl.
+  - simpl. destruct t0 as [s Hs].
+    rewrite inst_context_snoc /=. constructor; auto.
+    red. simpl. exists s.
+    eapply (Hs (Δ' ,,, inst_context σ Γ0) (⇑^#|Γ0| σ)) => //.
+    eapply well_subst_app; auto.
+  - simpl. destruct t0 as [s Hs]. simpl in t1.
+    rewrite inst_context_snoc /=. constructor; auto.
+    * simpl. exists s.
+      eapply (Hs (Δ' ,,, inst_context σ Γ0) (⇑^#|Γ0| σ)) => //.
+      eapply well_subst_app; auto.
+    * simpl. apply t1 => //.
+      eapply well_subst_app; eauto.
+Qed.
+
+Definition inst_constructor_body mdecl f c := 
+  map_constructor_body #|mdecl.(ind_params)| #|mdecl.(ind_bodies)|
+   (fun k => inst  (up k f)) c.
+
+Lemma inst_closed_decl k f d : closed_decl k d -> map_decl (inst (up k f)) d = d.
+Proof.
+  rewrite /closed_decl /map_decl.  
+  destruct d as [? [] ?] => /=.
+  - move/andP=> [] clt clty.
+    rewrite up_Upn !inst_closed //.
+  - move=> clt. rewrite !up_Upn !inst_closed //.
+Qed.
+
+Lemma inst_closed_constructor_body mdecl cdecl f : 
+  closed_constructor_body mdecl cdecl ->
+  inst_constructor_body mdecl f cdecl = cdecl.
+Proof.
+  rewrite /closed_constructor_body /inst_constructor_body /map_constructor_body.
+  move/andP=> [] /andP [] clctx clind clty.
+  destruct cdecl; cbn -[fold_context] in *; f_equal.
+  + move: clctx. unfold closed_ctx.
+    apply alli_fold_context => i d cldecl.
+    rewrite inst_closed_decl //.
+    red; rewrite -cldecl; lia_f_equal.
+  + solve_all. rewrite up_Upn inst_closed //.
+    red. rewrite -H0. lia_f_equal.
+  + now rewrite up_Upn inst_closed.
+Qed.
+
+Lemma inst_cstr_args mdecl f cdecl : 
+  cstr_args (inst_constructor_body mdecl f cdecl) =
+  inst_context (up (#|mdecl.(ind_params)| + #|ind_bodies mdecl|) f) (cstr_args cdecl).
+Proof. 
+  simpl. unfold inst_context.
+  apply fold_context_ext => i t.
+  now rewrite !up_Upn !Upn_Upn.
+Qed.
+
+Lemma inst_closedn_terms f n ts : 
+  forallb (closedn n) ts -> map (inst (up n f)) ts = ts.
+Proof.
+  solve_all. 
+  now rewrite up_Upn inst_closed.
+Qed.
+
+Lemma inst_closed_extended_subst f Γ : 
+  closed_ctx Γ ->
+  map (inst (up (context_assumptions Γ) f)) (extended_subst Γ 0) = extended_subst Γ 0. 
+Proof.
+  intros cl. apply inst_closedn_terms.
+  now apply (closedn_extended_subst_gen Γ 0 0).
+Qed.
+
+Lemma inst_lift :
+  forall f n k t,
+    inst (⇑^(n + k) f) (lift n k t) = lift n k (inst (⇑^k f) t).
+Proof.
+  intros f n k t.
+  rewrite !lift_rename.
+  autorewrite with sigma.
+  rewrite ren_lift_renaming.
+  eapply inst_ext.
+  rewrite -Upn_Upn Nat.add_comm Upn_Upn.
+  rewrite !Upn_compose.
+  apply Upn_ext. now rewrite shiftn_consn_idsn.
+Qed.
+
+Lemma inst_context_lift f n k Γ : 
+  inst_context (up (n + k) f) (lift_context n k Γ) =
+  lift_context n k (inst_context (up k f) Γ).
+Proof.
+  rewrite !inst_context_alt !lift_context_alt.
+  rewrite !mapi_mapi. apply mapi_ext => i x.
+  rewrite /lift_decl !compose_map_decl.
+  apply map_decl_ext => t; len.
+  generalize (Nat.pred #|Γ| - i).
+  intros.
+  rewrite !up_Upn -Upn_Upn.
+  rewrite (Nat.add_comm n k) Nat.add_assoc Nat.add_comm.
+  now rewrite inst_lift Upn_Upn.
+Qed.
+
+Lemma inst_inds f ind pu bodies : map (inst f) (inds ind pu bodies) = inds ind pu bodies.
+Proof.
+  unfold inds.
+  induction #|bodies|; simpl; auto. f_equal.
+  apply IHn.
+Qed.
+
+Lemma closed_ctx_args n bctx ctx : 
+  #|bctx| = #|ctx| ->
+  closedn_ctx n ctx ->
+  closedn_ctx n (map2 set_binder_name bctx ctx).
+Proof.
+  induction ctx in bctx |- *; destruct bctx; simpl; auto.
+  rewrite !closedn_ctx_cons => [=] hlen.
+  move/andP=> [cla clctx].
+  rewrite IHctx // /=.
+  rewrite map2_length //.
+  rewrite /closed_decl /= in clctx *. now rewrite hlen.
+Qed.
+
+Lemma inst_case_branch_context_gen ind mdecl f p bctx cdecl :
+  closedn_ctx (#|ind_params mdecl| + #|ind_bodies mdecl|)
+    (cstr_args cdecl) ->
+  closed_ctx (ind_params mdecl) ->
+  #|bctx| = #|cstr_args cdecl| ->
+  #|pparams p| = context_assumptions (ind_params mdecl) ->
+  inst_context f (case_branch_context ind mdecl p bctx cdecl) = 
+  case_branch_context ind mdecl (inst_predicate f p) bctx 
+    (inst_constructor_body mdecl f cdecl).
+Proof.
+  intros clargs clpars. unfold case_branch_context, case_branch_context_gen.
+  rewrite inst_cstr_args.
+  cbn -[fold_context].
+  intros hlen hlen'.
+  rewrite map2_set_binder_name_fold //.
+  change (fold_context
+  (fun i : nat => inst (up i (up (ind_npars mdecl + #|ind_bodies mdecl|) f)))) with
+    (inst_context (up (ind_npars mdecl + #|ind_bodies mdecl|) f)).
+  rewrite inst_context_subst. f_equal.
+  unfold id.
+  rewrite /expand_lets_ctx /expand_lets_k_ctx.
+  simpl. len.
+  rewrite inst_context_subst; len.
+  rewrite hlen'.
+  rewrite -{1}(context_assumptions_subst_instance_context (puinst p)).
+  rewrite -up_Upn.
+  rewrite inst_closed_extended_subst.
+  { now rewrite closedn_subst_instance_context. }
+  f_equal.
+  rewrite -Upn_Upn -up_Upn Nat.add_comm.
+  rewrite inst_context_lift. f_equal.
+  rewrite inst_context_subst_k inst_inds. len.
+  f_equal.
+  rewrite inst_closedn_ctx //.
+  * rewrite closedn_subst_instance_context.
+    now rewrite closed_ctx_args.
+  * rewrite -/(inst_context (up (#|ind_params mdecl| + #|ind_bodies mdecl|) f)
+      (map2 set_binder_name bctx (cstr_args cdecl))).
+    rewrite up_Upn inst_closedn_ctx //.
+    now rewrite closed_ctx_args.
+Qed.
+
+Lemma forallb_map_spec {A B : Type} {p : A -> bool}
+      {l : list A} {f g : A -> B} :
+  (forall x : A, p x -> f x = g x) -> 
+  forallb p l ->
+  map f l = map g l.
+Proof.
+  induction l; simpl; trivial.
+  rewrite andb_and. intros Hx [px pl].
+  f_equal. - now apply Hx. - now apply IHl.
+Qed.
+
+Lemma inst_case_branch_type {Σ} {wfΣ : wf Σ} f (ci : case_info) i mdecl idecl p br cdecl : 
+  declared_constructor Σ (ci.(ci_ind), i) mdecl idecl cdecl ->
+  wf_predicate mdecl idecl p ->
+  wf_branch cdecl br ->
+  let ptm := 
+    it_mkLambda_or_LetIn (case_predicate_context ci mdecl idecl p) (preturn p) 
+  in
+  let p' := inst_predicate f p in
+  let ptm' :=
+    it_mkLambda_or_LetIn
+      (case_predicate_context ci mdecl idecl p')
+      (preturn p') in
+  case_branch_type ci mdecl idecl
+     (inst_predicate f p) 
+     (map_branch (inst (up #|bcontext br| f)) br) 
+     ptm' i (inst_constructor_body mdecl f cdecl) =
+  map_pair (inst_context f) (inst (up #|bcontext br| f)) 
+  (case_branch_type ci mdecl idecl p br ptm i cdecl).
+Proof.
+  intros decli wfp wfb ptm p' ptm'.
+  rewrite /case_branch_type /case_branch_type_gen /map_pair /=.
+  rewrite inst_case_branch_context_gen //.
+  { epose proof (declared_constructor_closed_args decli). now rewrite Nat.add_comm. }
+  { eapply (declared_inductive_closed_params decli). }
+  { now apply wf_branch_length. }
+  { rewrite -(declared_minductive_ind_npars decli).
+    apply (wf_predicate_length_pars wfp). }
+  f_equal.
+  rewrite inst_mkApps map_app map_map_compose.
+  rewrite (wf_branch_length wfb).
+  f_equal.
+  * rewrite /ptm' /ptm !lift_it_mkLambda_or_LetIn !inst_it_mkLambda_or_LetIn.
+    rewrite !lift_rename. f_equal.
+    ++ rewrite /p'.
+      rewrite -(inst_case_predicate_context decli) //.
+      epose proof (inst_context_lift f #|cstr_args cdecl| 0).
+      rewrite Nat.add_0_r in H0.
+      rewrite H0. len. now rewrite up_Upn Upn_0.
+    ++ rewrite /p'. rewrite Nat.add_0_r. simpl.
+      rewrite case_predicate_context_length //.
+      { now apply inst_wf_predicate. }
+      rewrite !case_predicate_context_length // Nat.add_0_r; len.
+      rewrite case_predicate_context_length //.
+      rewrite !up_Upn -Upn_Upn. rewrite - !lift_rename.
+      now rewrite Nat.add_comm inst_lift.
+  * rewrite /= inst_mkApps /=. f_equal.
+    ++ rewrite !map_map_compose /id.
+      generalize (declared_constructor_closed_indicess decli).
+      apply forallb_map_spec => t clt.
+      rewrite !up_Upn.
+      rewrite /expand_lets /expand_lets_k.
+      rewrite -inst_subst_instance_constr. len.
+      rewrite inst_subst. f_equal.
+      rewrite inst_subst. rewrite (wf_predicate_length_pars wfp).
+      rewrite (declared_minductive_ind_npars decli).
+      rewrite -{2}(context_assumptions_subst_instance_context (puinst p) (ind_params mdecl)).
+      setoid_rewrite <- up_Upn at 1.
+      rewrite inst_closed_extended_subst.
+      { rewrite closedn_subst_instance_context.
+        apply (declared_inductive_closed_params decli). }
+      f_equal. len. rewrite - !Upn_Upn.
+      rewrite (Nat.add_comm _ (context_assumptions _)) inst_lift.
+      f_equal. rewrite Nat.add_comm inst_subst.
+      rewrite inst_inds. f_equal.
+      rewrite - Upn_Upn. len.
+      rewrite inst_closed ?closedn_subst_instance_constr //.
+      { rewrite Nat.add_comm.
+        now rewrite (Nat.add_comm #|cstr_args cdecl|) Nat.add_assoc. }
+      rewrite inst_closed. ?closedn_subst_instance_constr //.
+        { rewrite Nat.add_comm.
+          now rewrite (Nat.add_comm #|cstr_args cdecl|) Nat.add_assoc. }
+        
+    ++ unfold id. f_equal. f_equal.
+       rewrite map_app map_map_compose.
+       rewrite map_map_compose.
+       setoid_rewrite inst_shiftn. len. f_equal.
+       rewrite inst_to_extended_list.
+       now rewrite /to_extended_list /to_extended_list_k reln_fold.
+Qed.
 
 Lemma type_inst :
   forall Σ Γ Δ σ t A,
@@ -628,10 +980,17 @@ Proof.
   apply (typing_ind_env (fun Σ Γ t T => forall Δ σ,
     wf_local Σ Δ ->
     Σ ;;; Δ ⊢ σ : Γ ->
-    Σ ;;; Δ |- t.[σ] : T.[σ]
-  ) (fun Σ Γ wfΓ => forall Δ σ, wf_local Σ Δ ->    Σ ;;; Δ ⊢ σ : Γ ->
-      wf_local Σ Δ)).
+    Σ ;;; Δ |- t.[σ] : T.[σ])
+    (fun Σ Γ => 
+    All_local_env
+   (lift_typing (fun (Σ : global_env_ext) (Γ : context) (t T : term)
+    =>
+    forall Δ σ,
+    wf_local Σ Δ ->
+    Σ ;;; Δ ⊢ σ : Γ ->
+    Σ ;;; Δ |- t.[σ] : T.[σ]) Σ) Γ)).
   - intros Σ wfΣ Γ wfΓ. auto.
+    induction 1; constructor; firstorder auto.
     
   - intros Σ wfΣ Γ wfΓ n decl e X Δ σ hΔ hσ. simpl.
     eapply hσ. assumption.
@@ -695,12 +1054,66 @@ Proof.
     eapply meta_conv; [econstructor; eauto|].
     eapply declared_constructor_closed_type in isdecl; eauto.
     rewrite inst_closed0; eauto.
-  - intros Σ wfΣ Γ wfΓ ind u npar p c brs args mdecl idecl isdecl X X0 a pars
-           ps pty htoc X1 ihp H2 X3 notcoind ihc btys H3 ihbtys Δ σ hΔ hσ.
+  - intros Σ wfΣ Γ wfΓ ci p c brs indices ps mdecl idecl isdecl HΣ
+      IHΔ ci_npar predctx wfp Hpret IHpret IHpredctx isallowed
+      Hc IHc iscof ptm wfbrs Hbrs Δ f HΔ Hf.
     autorewrite with sigma. simpl.
     rewrite map_app. simpl.
-    rewrite map_skipn.
-    (* eapply types_of_case_inst with (σ := σ) in htoc. all: try eassumption. *)
+    rewrite /ptm. rewrite inst_it_mkLambda_or_LetIn.
+    relativize #|predctx|.
+    * erewrite inst_predicate_preturn.
+      rewrite /predctx.
+      rewrite (inst_case_predicate_context isdecl wfp).
+      eapply type_Case; eauto.
+      + now eapply inst_wf_predicate.
+      + apply All_local_env_app_inv in IHpredctx as [].
+        eapply IHpret.
+        ++ rewrite -inst_case_predicate_context //.
+           eapply wf_local_app_inst; eauto. apply a0.
+        ++ rewrite /predctx.
+           rewrite -{1}(case_predicate_context_length (ci:=ci) wfp).
+           rewrite -inst_case_predicate_context //.
+           eapply well_subst_app_up => //.
+           eapply wf_local_app_inst; eauto. apply a0.
+      + simpl. unfold id.
+        specialize (IHc _ _ HΔ Hf).
+        now rewrite inst_mkApps map_app in IHc.
+      + now eapply inst_wf_branches.
+      + eapply Forall2_All2 in wfbrs.
+        eapply All2i_All2_mix_left in Hbrs; eauto.
+        eapply All2i_nth_hyp in Hbrs.
+        eapply All2i_map_right, (All2i_impl Hbrs) => i cdecl br.
+        set (brctxty := case_branch_type _ _ _ _ _ _ _ _).
+        move=> [Hnth [wfbr [[Hbr Hbrctx] [IHbr [Hbty IHbty]]]]].
+        rewrite -(inst_closed_constructor_body mdecl cdecl f).
+        { eapply (declared_constructor_closed (c:=(ci.(ci_ind),i))); eauto.
+          split; eauto. }
+        rewrite inst_case_branch_type //.
+        rewrite -/brctxty. intros brctx'.
+        assert (wf_local Σ (Δ,,, brctx'.1)).
+        { rewrite /brctx'. cbn.
+          apply All_local_env_app_inv in Hbrctx as [].
+          eapply wf_local_app_renaming; tea. apply a0. }
+        repeat split.
+        ++ eapply IHbr. 
+          split => //.
+          rewrite /brctx' /brctxty; cbn.
+          rewrite (wf_branch_length wfbr).
+          erewrite <- case_branch_type_length; eauto.
+          eapply urenaming_ext.
+          { now rewrite app_context_length -shiftnP_add. }
+          { reflexivity. }
+          eapply urenaming_context, Hf.
+        ++ eapply IHbty. split=> //.
+          rewrite /brctx'; cbn.
+          rewrite (wf_branch_length wfbr).
+          erewrite <- case_branch_type_length; eauto.
+          eapply urenaming_ext.
+          { now rewrite app_context_length -shiftnP_add. }
+          { reflexivity. }
+          eapply urenaming_context, Hf.
+    * rewrite /predctx case_predicate_context_length //.
+
     eapply type_Case.
     + eassumption.
     + assumption.
