pcuic/theories/PCUICWeakening.v
@@ -4,7 +4,7 @@ From MetaCoq.Template Require Import config utils.
 From MetaCoq.PCUIC Require Import PCUICAst PCUICAstUtils PCUICCases PCUICInduction
   PCUICLiftSubst PCUICUnivSubst PCUICEquality PCUICTyping PCUICWeakeningEnv
   PCUICClosed PCUICReduction PCUICPosition PCUICGeneration
-  PCUICSigmaCalculus PCUICRename.
+  PCUICSigmaCalculus PCUICRename PCUICOnFreeVars.
 
 Require Import ssreflect ssrbool.
 From Equations Require Import Equations.
@@ -16,19 +16,11 @@ Implicit Types cf : checker_flags.
   [weakening_*] proves weakening of typing, reduction etc... w.r.t. the *local*
   environment. *)
 
-
 Set Default Goal Selector "!".
 Generalizable Variables Σ Γ t T.
 
-Derive Signature NoConfusion for All_local_env.
-Derive Signature for All_local_env_over.
-
 (* FIXME inefficiency in equations: using a very slow "pattern_sigma" to simplify an equality between sigma types *)
 Ltac Equations.CoreTactics.destruct_tele_eq H ::= noconf H.
-
-(* Derive Signature NoConfusion for All_local_env. *)
-(* Derive NoConfusion for All_local_env_over. *)
-(* Derive NoConfusion for context_decl. *)
 
 Lemma typed_liftn `{checker_flags} Σ Γ t T n k :
   wf Σ.1 -> wf_local Σ Γ -> k >= #|Γ| ->
@@ -100,77 +92,12 @@ Proof.
   rewrite permute_lift; try easy.
 Qed.
 
-Definition noccur_between_decl k n d :=
-  option_default (noccur_between k n) d.(decl_body) true && 
-  noccur_between k n d.(decl_type).
-
-Definition noccur_between_ctx k n (t : context) : bool :=
-  alli (fun k' => noccur_between_decl (k + k') n) 0 (List.rev t).
-
-Lemma noccur_between_ctx_cons k n d Γ : 
-  noccur_between_ctx k n (d :: Γ) = 
-  noccur_between_decl (k + #|Γ|) n d && noccur_between_ctx k n Γ.
-Proof.
-  unfold noccur_between_ctx.
-  simpl. rewrite alli_app /= andb_true_r.
-  now rewrite Nat.add_0_r List.rev_length andb_comm.
-Qed.
 
 Lemma All_local_env_eq P ctx ctx' :
   All_local_env P ctx -> 
   ctx = ctx' ->
   All_local_env P ctx'.
 Proof. now intros H ->. Qed.
-
-Lemma shiftn_ext_noccur_between f f' k n k' i :
-  (i < k' + k \/ k' + k + n <= i) ->
-  (forall i, i < k \/ k + n <= i -> f i = f' i) ->
-  shiftn k' f i = shiftn k' f' i.
-Proof.
-  intros.
-  unfold shiftn. destruct (Nat.ltb_spec i k').
-  - auto.
-  - rewrite H0; auto. lia.
-Qed.
-
-Lemma rename_ext_cond f f' k n : (forall i, i < k \/ k + n <= i -> f i = f' i) -> 
-  (forall t, noccur_between k n t -> rename f t = rename f' t).
-Proof.
-intros. revert k n t H0 f f' H.
-apply: term_noccur_between_list_ind; simpl in |- *; intros; try easy ;
-  try (try rewrite H; try rewrite H0 ; try rewrite H1 ; easy);
-  try solve [f_equal; solve_all].
-- f_equal; auto. apply H0. intros.
-  eapply (shiftn_ext_noccur_between f f' k n); eauto.
-- f_equal; auto. apply H0. intros.
-  eapply (shiftn_ext_noccur_between f f' k n); eauto.
-- f_equal; auto. eapply H1. intros.
-  eapply (shiftn_ext_noccur_between f f' k n); eauto.
-- destruct X. f_equal; auto; solve_all.
-  * apply e. intros.
-    eapply (shiftn_ext_noccur_between f f' k n); eauto.
-  * apply map_branch_eq_spec. apply H1.
-    intros; eapply (shiftn_ext_noccur_between f f' k n); eauto.
-- red in X. f_equal; solve_all.
-  eapply map_def_eq_spec; auto. apply b.
-  rewrite fix_context_length.
-  intros; eapply (shiftn_ext_noccur_between f f' k n); eauto.
-- f_equal; auto. red in X. solve_all.
-  eapply map_def_eq_spec; auto. apply b.
-  rewrite fix_context_length.
-  intros. eapply (shiftn_ext_noccur_between f f' k n); eauto.
-Qed.
-
-Lemma rename_decl_ext_cond f f' k n : (forall i, i < k \/ k + n <= i -> f i = f' i) -> 
-  (forall t, noccur_between_decl k n t -> rename_decl f t = rename_decl f' t).
-Proof.
-  intros Hi d. move/andb_and=> [clb clt].
-  rewrite /rename_decl.
-  destruct d as [na [b|] ty] => /=; rewrite /map_decl /=; simpl in *; f_equal.
-  - f_equal. now eapply rename_ext_cond.
-  - now eapply rename_ext_cond.
-  - now eapply rename_ext_cond.
-Qed.  
 
 Hint Rewrite shiftn_rshiftk : sigma.
 
@@ -241,458 +168,12 @@ Proof.
     constructor. lia.
 Qed.
 
-Definition strengthen k n :=
-  fun i => if i <? k then i else (i - n).
-
-Lemma shiftn_strengthen_rel k n i k' : 
-  (i < k + k' \/ k + k' + n <= i) ->
-  shiftn k (strengthen k' n) i = strengthen (k + k') n i.
-Proof.
-  rewrite /shiftn /strengthen.
-  destruct (Nat.ltb_spec i k); auto.
-  - destruct (Nat.ltb_spec i (k + k')); lia.
-  - destruct (Nat.ltb_spec (i - k) k'); destruct (Nat.ltb_spec i (k + k')); lia.
-Qed.
-
-Lemma shiftn_strengthen k k' n t : 
-  noccur_between (k' + k) n t ->
-  rename (shiftn k (strengthen k' n)) t = rename (strengthen (k + k') n) t.
-Proof.
-  intros nocc.
-  eapply rename_ext_cond; tea.
-  intros. eapply shiftn_strengthen_rel. lia.
-Qed.
-
-Definition strengthen_context (Γ Γs Δ : context) :=
-  Γ ,,, rename_context (strengthen 0 #|Γs|) Δ.
-
-Definition strengthen_rename Δ Γs i :=  
-  if i <? Δ then
-    strengthen (Δ - S i) Γs
-  else id.
-
-Lemma map_decl_id : map_decl id =1 id.
-Proof. intros d; now destruct d as [? [] ?]. Qed.
-
-
-Lemma lookup_strengthen_context Γ Γs Δ i :
-  let Δ' := lift_context #|Γs| 0 Δ in 
-  nocc_betweenp #|Δ| #|Γs| i ->
-  nth_error (strengthen_context Γ Γs Δ') (strengthen #|Δ| #|Γs| i) = 
-  option_map (map_decl (rename (strengthen_rename #|Δ| #|Γs| i))) 
-    (nth_error (Γ ,,, Γs ,,, Δ') i).
-Proof.
-  simpl.
-  rewrite /strengthen_context /strengthen /nocc_betweenp.
-  (* Again, => _ is counter-intuitive to me here. e.g when doing
-    repeat (nat_compare_specs => /= //) => /= _. it's not equivalent
-    to the line below.
-   *)
-  repeat (nat_compare_specs => /= //). all:move=> _.
-  * rewrite (nth_error_app_context_ge i); len => //.
-    rewrite (nth_error_app_context_ge (i - #|Δ|)); len; try lia => //.
-    rewrite (nth_error_app_context_ge (i - #|Γs|)); len; try lia => //.
-    replace (i - #|Δ| - #|Γs|) with (i - #|Γs| - #|Δ|) by lia.
-    destruct nth_error => /= //. f_equal.
-    rewrite -{1}[c](map_decl_id c).
-    apply map_decl_ext => x.
-    rewrite -(rename_ren_id x).
-    apply rename_ext.
-    rewrite /strengthen_rename. nat_compare_specs.
-    reflexivity.
-  * rewrite nth_error_app_lt; len => //.
-    rewrite nth_error_app_lt; len => //.
-    rewrite /rename_context.
-    rewrite nth_error_lift_context_eq Nat.add_0_r.
-    rewrite /lift_context fold_context_compose option_map_two.
-    destruct (nth_error Δ i) eqn:hnth => //.
-    + rewrite (nth_error_fold_context _ _ _ _ _ _ hnth) /=; eauto.
-      f_equal. rewrite compose_map_decl. apply map_decl_ext => t.
-      rewrite !lift_rename !rename_compose.
-      eapply rename_ext => k.
-      rewrite /strengthen_rename /shiftn /lift_renaming /= /strengthen.
-      now repeat nat_compare_specs => /= //.
-    + now apply nth_error_None in hnth.
-Qed.
-
-Lemma strengthen_shiftn k n : strengthen k n ∘ (shiftn k (rshiftk n)) =1 id.
-Proof.
-  intros i; rewrite /strengthen /shiftn /rshiftk /id.
-  repeat nat_compare_specs.
-Qed.
-
-Lemma rshiftk_shiftn k n l i : rshiftk k (shiftn n l i) = shiftn (n + k) l (rshiftk k i).
-Proof.
-  intros.
-  rewrite /rshiftk. 
-  rewrite /shiftn. repeat nat_compare_specs.
-  replace (k + i - (n + k)) with (i - n) by lia. lia.
-Qed.
-
-Lemma S_rshiftk k n : S (rshiftk k n) = rshiftk (S k) n.
-Proof. reflexivity. Qed.
-
-Lemma strengthen_lift_renaming n k i : strengthen k n (lift_renaming n k i) = i.
-Proof.
-  rewrite /strengthen /lift_renaming.
-  repeat nat_compare_specs.
-Qed.
-
-Lemma strengthen_lift n k t : rename (strengthen k n) (lift n k t) = t.
-Proof.
-  rewrite lift_rename rename_compose.
-  setoid_rewrite strengthen_lift_renaming.
-  now rewrite rename_ren_id.
-Qed.
-
 Lemma rename_context_lift_context n k Γ :
   rename_context (lift_renaming n k) Γ = lift_context n k Γ.
 Proof.
   rewrite /rename_context /lift_context.
   apply fold_context_ext => i t.
   now rewrite lift_rename shiftn_lift_renaming.
-Qed.
-
-Lemma shiftn_id i : shiftn i id =1 id.
-Proof. intros k; rewrite /shiftn. nat_compare_specs => /= //.
-  rewrite /id. lia.
-Qed.
-
-Lemma fold_context_id x : fold_context (fun i x => x) x = x.
-Proof.
-  rewrite fold_context_alt.
-  rewrite /mapi. generalize 0.
-  induction x; simpl; auto.
-  intros n.
-  f_equal; auto. 
-  now rewrite map_decl_id.
-Qed.
-
-Lemma strengthen_lift_ctx n k t : rename_context (strengthen k n) (lift_context n k t) = t.
-Proof.
-  rewrite -rename_context_lift_context.
-  rewrite /rename_context fold_context_compose.
-  rewrite -{2}(fold_context_id t).
-  apply fold_context_ext => i x.
-  rewrite rename_compose shiftn_compose.  
-  setoid_rewrite strengthen_lift_renaming.
-  now rewrite shiftn_id rename_ren_id.
-Qed.
-
-Lemma strengthen_urenaming_gen Γ Γs Δ :
-  let Δ' := lift_context #|Γs| 0 Δ in 
-  urenaming (nocc_betweenp #|Δ| #|Γs|)
-    (strengthen_context Γ Γs Δ')
-    (Γ ,,, Γs ,,, Δ')
-    (strengthen #|Δ| #|Γs|).
-Proof.
-  intros Δ' i d hpi hnth.
-  rewrite lookup_strengthen_context /= // hnth /=.
-  eexists; split; eauto.
-  destruct d as [na b ty]; simpl in *.
-  unfold nocc_betweenp in hpi.
-  move/orP: hpi. intros hi.
-  move: hnth. rewrite /Δ'.
-  move: hi => []; [move/Nat.ltb_lt|move/Nat.leb_le] => hi.
-  - rewrite nth_error_app_context_lt; len; try lia.
-    rewrite nth_error_lift_context_eq Nat.add_0_r.
-    destruct nth_error eqn:hnth => /= // [=] <- <- <-.
-    repeat split.
-    + rewrite rename_compose lift_rename !rename_compose.
-      apply rename_ext.
-      intros k. 
-      change (S (rshiftk i (lift_renaming #|Γs| (#|Δ| - S i) k)))
-        with (rshiftk (S i) (lift_renaming #|Γs| (#|Δ| - S i) k)).
-      rewrite lift_renaming_spec.
-      rewrite /strengthen_rename. nat_compare_specs.
-      rewrite (strengthen_shiftn _ _ _) /id.
-      rewrite rshiftk_shiftn Nat.sub_add // S_rshiftk.
-      rewrite -lift_renaming_spec strengthen_lift_renaming.
-      rewrite /strengthen. nat_compare_specs.
-    + destruct (decl_body c) => /= //.
-      f_equal.
-      rewrite rename_compose lift_rename !rename_compose.
-      apply rename_ext.
-      intros k. 
-      change (S (rshiftk i (lift_renaming #|Γs| (#|Δ| - S i) k)))
-        with (rshiftk (S i) (lift_renaming #|Γs| (#|Δ| - S i) k)).
-      rewrite lift_renaming_spec.
-      rewrite /strengthen_rename. nat_compare_specs.
-      rewrite (strengthen_shiftn _ _ _) /id.
-      rewrite rshiftk_shiftn Nat.sub_add // S_rshiftk.
-      rewrite -lift_renaming_spec strengthen_lift_renaming.
-      rewrite /strengthen. nat_compare_specs.
-  - rewrite nth_error_app_context_ge; len; try lia.
-    rewrite nth_error_app_context_ge; len; try lia.
-    intros hnth.
-    repeat split.
-    + rewrite !rename_compose.
-      apply rename_ext => k.
-      rewrite /strengthen /strengthen_rename /rshiftk /id.
-      repeat nat_compare_specs.
-    + destruct b => //. simpl. f_equal.
-      rewrite !rename_compose.
-      apply rename_ext => k.
-      rewrite /strengthen /strengthen_rename /rshiftk /id.
-      repeat nat_compare_specs.
-Qed.
-
-Lemma strengthen_urenaming Γ Γs Δ :
-  let Δ' := lift_context #|Γs| 0 Δ in 
-  urenaming (nocc_betweenp #|Δ| #|Γs|)
-    (Γ ,,, Δ)
-    (Γ ,,, Γs ,,, Δ')
-    (strengthen #|Δ| #|Γs|).
-Proof.
-  pose proof (strengthen_urenaming_gen Γ Γs Δ).
-  simpl in X.
-  rewrite /strengthen_context in X.
-  now rewrite strengthen_lift_ctx in X.
-Qed.
-
-(* l, r, p -> r, l, p *)
-Definition exchange_renaming l r p :=
-  fun i => 
-    if p <=? i then
-      if p + r <=? i then
-        if p + r + l <=? i then i
-        else i - r
-      else i + l
-    else i.
-
-Variant exchange_renaming_spec l r p i : nat -> Type :=
-| exch_below : i < p -> exchange_renaming_spec l r p i i
-| exch_right : p <= i < p + r -> exchange_renaming_spec l r p i (i + l)
-| exch_left : p + r <= i < p + r + l -> exchange_renaming_spec l r p i (i - r)
-| exch_above : p + r + l <= i -> exchange_renaming_spec l r p i i.
-
-Lemma exchange_renamingP l r p i : 
-  exchange_renaming_spec l r p i (exchange_renaming l r p i).
-Proof.
-  unfold exchange_renaming.
-  case: leb_spec_Set; [|constructor; auto].
-  elim: leb_spec_Set; [|constructor; auto].
-  elim: leb_spec_Set; [|constructor; auto].
-  intros.
-  constructor 4; auto.
-Qed.
-
-Lemma shiftn_exchange_renaming n l r p : 
-  shiftn n (exchange_renaming l r p) =1 
-  exchange_renaming l r (n + p).
-Proof.
-  intros i.
-  case: exchange_renamingP.
-  * case: shiftnP; try lia.
-    case: exchange_renamingP; lia.
-  * case: shiftnP; try lia.
-    case: exchange_renamingP; lia.
-  * case: shiftnP; try lia.
-    case: exchange_renamingP; lia.
-  * case: shiftnP; try lia.
-    case: exchange_renamingP; lia.
-Qed.
-
-Lemma exchange_renaming_lift_renaming l r p i k :
-  i < p ->
-  exchange_renaming l r p (lift_renaming (S i) 0 k) =
-  lift_renaming (S i) 0
-    (shiftn (p - S i) (exchange_renaming l r 0) k).
-Proof.
-  intros ip.
-  rewrite shiftn_exchange_renaming.
-  rewrite /lift_renaming /=.
-  case: exchange_renamingP; try lia; intros Hp.
-  all: case: exchange_renamingP; lia.
-Qed.
-
-Definition exchange_contexts Γ Γl Γr Δ :=
-  (Γ ,,, rename_context (strengthen 0 #|Γl|) Γr ,,, 
-  rename_context (lift_renaming #|Γr| 0) Γl ,,, 
-  rename_context (exchange_renaming #|Γl| #|Γr| 0) Δ).
-
-Definition exchange_rename Γl Γr Δ i :=
-  if Δ <=? i then
-    if Δ + Γr <=? i then
-      if Δ + Γr + Γl <=? i then ren_id
-      else (lift_renaming Γr (Γl - S (i - Γr - Δ)))
-    else (shiftn (Γr - S (i - Δ)) (strengthen 0 Γl))
-  else (exchange_renaming Γl Γr (Δ - S i)).
-
-Instance option_map_ext {A B} : Proper (`=1` ==> Logic.eq ==> Logic.eq) (@option_map A B).
-Proof.
-  intros f g Hfg x y <-.
-  now destruct x => /=; f_equal.
-Qed.
-
-Lemma option_map_id {A} : option_map (@id A) =1 id.
-Proof. by intros []. Qed.
-
-Instance map_decl_pointwise : Proper (`=1` ==> `=1`) map_decl.
-Proof. intros f g Hfg x. rewrite /map_decl.
-  destruct x => /=. f_equal.
-  - now rewrite Hfg.
-  - apply Hfg.
-Qed.
-
-Lemma lookup_exchange_contexts Γ Γl Γr Δ i :
-  nth_error (exchange_contexts Γ Γl Γr Δ) (exchange_renaming #|Γl| #|Γr| #|Δ| i) =
-  option_map (map_decl (rename (exchange_rename #|Γl| #|Γr| #|Δ| i))) 
-    (nth_error (Γ ,,, Γl,,, Γr,,, Δ) i).
-Proof.
-  rewrite /exchange_renaming /exchange_contexts /exchange_rename.
-  case: (leb_spec_Set #|Δ| i) => hΔ.
-  * case: leb_spec_Set => hΓr.
-    + case: leb_spec_Set => hΓl.
-      - do 6 (rewrite nth_error_app_ge; len; try lia => //).
-        assert (i - #|Δ| - #|Γl| - #|Γr| = i - #|Δ| - #|Γr| - #|Γl|) as -> by lia.
-        now rewrite rename_ren_id map_decl_id option_map_id.
-      - rewrite nth_error_app_ge; len; try lia => //.
-        rewrite nth_error_app_lt; len; try lia => //.
-        rewrite nth_error_app_ge; len; try lia => //.
-        rewrite nth_error_app_ge; len; try lia => //.
-        rewrite nth_error_app_lt; len; try lia => //.
-        rewrite nth_error_rename_context.
-        assert (i - #|Δ| - #|Γr| = i - #|Γr| - #|Δ|) as -> by lia.
-        apply option_map_ext => //.
-        intros d. apply map_decl_ext => t.
-        now rewrite shiftn_lift_renaming Nat.add_0_r.
-    + rewrite nth_error_app_ge; len; try lia => //.
-      rewrite nth_error_app_ge; len; try lia => //.
-      rewrite nth_error_app_lt; len; try lia => //.
-      rewrite nth_error_app_ge; len; try lia => //.
-      rewrite nth_error_app_lt; len; try lia => //.
-      rewrite nth_error_rename_context.
-      assert (i + #|Γl| - #|Δ| - #|Γl| = i - #|Δ|) as -> by lia.
-      reflexivity.
-  * rewrite nth_error_app_lt; len; try lia => //.
-    rewrite nth_error_app_lt; len; try lia => //.
-    rewrite nth_error_rename_context.
-    now rewrite shiftn_exchange_renaming Nat.add_0_r.
-Qed.
-
-
-(* 
-Lemma exchange_renaming_add Γl Γr Δ n : 
-  exchange_renaming Γl Γr Δ n = n + exchange_renaming Γl Γr Δ 0.
-Proof.
-  case: exchange_renamingP; case: exchange_renamingP; simpl; try lia.
-  - intros.
- *)
- 
-Lemma exchange_rename_Δ Γl Γr Δ i (k : nat) :
-  (* noccur_between_ctx 0 Γl Γr -> *)
-  i < Δ ->
-  (* From the i-prefix of Γ Γl Γr Δ to Γ Γr Γl Δ *)
-  exchange_renaming Γl Γr Δ (S i + k) = 
-  S (i + exchange_renaming Γl Γr (Δ - S i) k).
-Proof.
-  rewrite /exchange_renaming.
-  repeat nat_compare_specs; lia.
-Qed.
-
-Lemma exchange_rename_Γr Γl Γr Δ i (k : nat) :
-  (* noccur_between_ctx 0 Γl Γr -> *)
-  Δ <= i < Δ + Γr ->
-  k < Γr - S (i - Δ) \/ Γr - S (i - Δ) + Γl <= k ->
-  (* From the i-prefix of Γ Γl Γr Δ to Γ Γr Γl Δ *)
-  exchange_renaming Γl Γr Δ (S i + k) = 
-  S (i + Γl + strengthen (Γr - S (i - Δ)) Γl k).
-Proof.
-  rewrite /exchange_renaming /strengthen.
-  repeat nat_compare_specs.
-Qed.
-(* 
-Lemma exchange_rename_Γl Γl Γr Δ i (k : nat) :
-  (* noccur_between_ctx 0 Γl Γr -> *)
-  Δ + Γr <= i < Δ + Γr + Γl ->
-  (* From the i-prefix of Γ Γl Γr Δ to Γ Γr Γl Δ *)
-  exchange_renaming Γl Γr Δ (S i + k) = 
-  S (i + exchange_renaming Γl Γr (Δ - S i) k).
-Proof.
-  rewrite /exchange_renaming.
-  repeat nat_compare_specs; lia.
-Qed. *)
-
-
-Lemma nth_error_noccur_between_ctx k n Γ i d : 
-  noccur_between_ctx k n Γ -> 
-  nth_error Γ i = Some d ->
-  noccur_between_decl (k + (#|Γ| - S i)) n d.
-Proof.
-  rewrite /noccur_between_ctx.
-  intros alli nth. apply alli_Alli in alli.
-  eapply Alli_rev_nth_error in alli; eauto.
-Qed.
-
-Lemma exchange_lift_rename {Γ Γl Γr Δ : context} {i d} :
-  noccur_between_ctx 0 #|Γl| Γr ->
-  nth_error (Γ,,, Γl,,, Γr,,, Δ) i = Some d ->
-  rename_decl (fun k => exchange_renaming #|Γl| #|Γr| #|Δ| (S (i + k))) d =
-  rename_decl (fun k => S (exchange_renaming #|Γl| #|Γr| #|Δ| i + exchange_rename #|Γl| #|Γr| #|Δ| i k)) d.
-Proof.
-  intros nocc hlen.
-  move: hlen.
-  case: lookup_declP => // d' Hi hnth [=]; intros ->; [|move: hnth; len in Hi].
-  { apply map_decl_ext, rename_ext => k.
-    rewrite {2}/exchange_renaming /exchange_rename. nat_compare_specs.
-    now apply exchange_rename_Δ. }
-  case: lookup_declP => // d' Hi' hnth [=]; intros ->; [|move: hnth; len in Hi'].
-  { eapply nth_error_noccur_between_ctx in nocc; eauto.
-    simpl in nocc. move: nocc.
-    apply rename_decl_ext_cond => k Hk.
-    rewrite {2}/exchange_renaming /exchange_rename.
-    repeat nat_compare_specs.
-    rewrite shiftn_strengthen_rel Nat.add_0_r //.
-    now rewrite exchange_rename_Γr. }
-  case: lookup_declP => // d' Hi'' hnth [=]; intros ->; [|move: hnth; len in Hi''].
-  { apply map_decl_ext, rename_ext => k.
-    rewrite /exchange_renaming /exchange_rename /lift_renaming; 
-    repeat nat_compare_specs. }
-  { move/nth_error_Some_length => hlen.
-    apply map_decl_ext, rename_ext => k.
-    rewrite /exchange_renaming /exchange_rename; repeat nat_compare_specs.
-    now unfold ren_id. }
-Qed.
-
-Lemma exchange_urenaming P Γ Γl Γr Δ :
-  noccur_between_ctx 0 #|Γl| Γr ->
-  urenaming P
-    (exchange_contexts Γ Γl Γr Δ)
-    (Γ ,,, Γl ,,, Γr ,,, Δ)
-    (exchange_renaming #|Γl| #|Γr| #|Δ|).
-Proof.
-  intros nocc i d hpi hnth.
-  rewrite lookup_exchange_contexts hnth => /=.
-  eexists; split; eauto.
-  pose proof (exchange_lift_rename nocc hnth).
-  rewrite !rename_compose /lift_renaming /=. 
-  destruct d as [na [b|] ty]; noconf H; simpl in *.
-  - split => //.
-    split => //.
-    f_equal.
-    rewrite !rename_compose.
-    rewrite /lift_renaming /= //. 
-  - split => //.
-Qed.
-
-Lemma All_local_env_fold P f Γ :
-  All_local_env (fun Γ t T => P (fold_context f Γ) (f #|Γ| t) (option_map (f #|Γ|) T)) Γ <~>
-  All_local_env P (fold_context f Γ).
-Proof.
-  split.
-  - induction 1; simpl; rewrite ?fold_context_snoc0; constructor; auto.
-  - induction Γ; simpl; rewrite ?fold_context_snoc0; intros H.
-    * constructor.
-    * destruct a as [na [b|] ty]; depelim H; specialize (IHΓ H); constructor; auto.
-Qed.
-
-Lemma All_local_env_impl_ind {P Q : context -> term -> option term -> Type} {l} :
-  All_local_env P l ->
-  (forall Γ t T, All_local_env Q Γ -> P Γ t T -> Q Γ t T) ->
-  All_local_env Q l.
-Proof.
-  induction 1; intros; simpl; econstructor; eauto.
 Qed.
 
 Lemma weakening_wf_local {cf: checker_flags} {Σ : global_env_ext} {wfΣ : wf Σ} {Γ Γ' Γ''} :
@@ -734,6 +215,21 @@ Proof.
   intros ? ? ->; now apply weakening_wf_local.
 Qed.
 
+Lemma weakening_rename_typing `{cf : checker_flags} {Σ : global_env_ext} {wfΣ : wf Σ} {Γ Γ' Γ''} {t T} :
+  wf_local Σ (Γ ,,, Γ'') ->
+  Σ ;;; Γ ,,, Γ' |- t : T ->
+  Σ ;;; Γ ,,, Γ'' ,,, rename_context (lift_renaming #|Γ''| 0) Γ' |- 
+    rename (lift_renaming #|Γ''| #|Γ'|) t : 
+    rename (lift_renaming #|Γ''| #|Γ'|) T.
+Proof.
+  intros wfext Ht.
+  eapply (typing_rename); eauto.
+  rewrite rename_context_lift_context.
+  split.
+  - eapply weakening_wf_local; eauto with pcuic.
+  - now apply weakening_renaming.
+Qed.
+
 Lemma weakening_typing `{cf : checker_flags} {Σ : global_env_ext} {wfΣ : wf Σ} {Γ Γ' Γ''} {t T} :
   wf_local Σ (Γ ,,, Γ'') ->
   Σ ;;; Γ ,,, Γ' |- t : T ->
@@ -769,661 +265,6 @@ Proof.
   now eapply closed_wf_local.
 Qed.
 
-Lemma wf_local_app_ind {cf : checker_flags} {Σ Γ1 Γ2} :
-  wf_local Σ Γ1 -> 
-  (wf_local Σ Γ1 -> wf_local_rel Σ Γ1 Γ2) ->
-  wf_local Σ (Γ1 ,,, Γ2).
-Proof.
-  intros wf IH.
-  apply wf_local_app; auto.
-Qed.
-
-Lemma meta_conv_all {cf} {Σ Γ t A Γ' t' A'} :
-    Σ ;;; Γ |- t : A ->
-    Γ = Γ' -> t = t' -> A = A' ->
-    Σ ;;; Γ' |- t' : A'.
-Proof.
-  intros h [] [] []; assumption.
-Qed.
-
-Instance fold_context_proper : Proper (pointwise_relation nat (pointwise_relation _ Logic.eq) ==> Logic.eq ==> Logic.eq) fold_context.
-Proof.
-  intros f g Hfg x y <-. now apply fold_context_ext.
-Qed.
-
-Definition isLift n k t := 
-  ∑ t', t = lift n k t'.
-
-Lemma isLift_rel n k i : 
-  isLift n k (tRel i) -> nocc_betweenp k n i.
-Proof.
-  intros [t' eq]. destruct t' => //.
-  simpl in eq. noconf eq.
-  unfold nocc_betweenp.
-  repeat nat_compare_specs => /= //.
-Qed.
-
-Lemma All_local_env_over_simpl {cf:checker_flags} Σ Γ : 
-  forall wfΓ : wf_local Σ Γ, 
-  All_local_env_over typing
-  (fun (Σ : global_env_ext) (Γ : context) (_ : wf_local Σ Γ)
-    (t T : term) (_ : Σ;;; Γ |- t : T) =>
-  forall Γl Γs Δ : context,
-  Γ = Γl,,, Γs,,, lift_context #|Γs| 0 Δ ->
-  isLift #|Γs| #|Δ| t ->
-  isLift #|Γs| #|Δ| T ->
-  Σ;;; Γl,,, Δ |- rename (strengthen #|Δ| #|Γs|) t
-  : rename (strengthen #|Δ| #|Γs|) T) Σ Γ wfΓ ->
-  All_local_env
-  (lift_typing (fun (Σ : global_env_ext) (Γ : context) (t T : term)  =>
-  forall Γl Γs Δ : context,
-  Γ = Γl,,, Γs,,, lift_context #|Γs| 0 Δ ->
-  isLift #|Γs| #|Δ| t ->
-  isLift #|Γs| #|Δ| T ->
-  Σ;;; Γl,,, Δ |- rename (strengthen #|Δ| #|Γs|) t
-  : rename (strengthen #|Δ| #|Γs|) T) Σ) Γ.
-Proof.
-  intros wfΓ. unfold lift_typing.
-  induction 1; constructor; intuition auto.
-  - destruct tu as [s Hs]; exists s; intuition auto.
-  - destruct tu as [s Hs]; exists s; intuition auto.
-Qed.
-
-Lemma isLift_lift n k t : isLift n k (lift n k t).
-Proof. eexists; eauto. Qed.
-
-Definition is_strengthenable {cf:checker_flags} {Σ Γ t T} (d : Σ ;;; Γ |- t : T) (k n : nat) : bool.
-Proof.
-  revert Γ t T d k.
-  fix aux 4.
-  intros. destruct d.
-  - exact (nocc_betweenp k n n0).
-  - exact true.
-  - exact (aux _ _ _ d1 k && aux _ _ _ d2 (S k)).
-  - exact (aux _ _ _ d1 k && aux _ _ _ d2 (S k)).
-  - exact [&& aux _ _ _ d1 k, aux _ _ _ d2 k & aux _ _ _ d3 (S k)].
-  - exact [&& aux _ _ _ d1 k, aux _ _ _ d2 k & aux _ _ _ d3 k].
-  - exact true.
-  - exact true.
-  - exact true.
-  - exact true.
-  - exact true.
-  - exact true.
-  - exact true.
-  - exact (aux _ _ _ d1 k && aux _ _ _ d2 k).
-Defined.
-
-Lemma is_strengthenable_isLift {cf:checker_flags} {Σ Γ t T} (d : Σ ;;; Γ |- t : T) {n k}:
-  is_strengthenable d k n ->
-  isLift n k t × isLift n k T.
-Proof.
-  induction d in n, k |- *; simpl; intros.
-  - admit.
-  - split; eexists (tSort _); simpl; eauto.
-  - move/andP: H => [isd1 isd2].
-    specialize (IHd1 _ _ isd1) as [[A' ->] _].
-    specialize (IHd2 _ _ isd2) as [[B' ->] _].
-    split.
-    * eexists (tProd na _ _); simpl; eauto.
-    * now eexists (tSort _).
-  - admit.
-  - admit.
-  - move/and3P: H => [hd1 hd2 hd3].
-    specialize (IHd1 _ _ hd1) as [[p' eq] _].
-    specialize (IHd2 _ _ hd2) as [[? ->] _].
-    specialize (IHd3 _ _ hd3) as [[? ->] ?].
-    split.
-    * now eexists (tApp _ _).
-    * destruct p' => //.
-      noconf eq.
-      rewrite /subst1.
-      rewrite -(distr_lift_subst_rec _ [_]) /=.
-      now eexists _.
-  - split.
-    * now eexists (tConst _ _).
-    * admit.
-  - admit.
-  - admit.
-  - admit.
-  - admit.
-  - admit.
-  - admit.
-  - move/andP: H => [hd1 hd2].
-    split.
-    * apply (IHd1 _ _ hd1).
-    * eapply (IHd2 _ _ hd2).
-Admitted.
-
-(** For an unconditional renaming defined on all variables in the source context *)
-Lemma typing_rename_prop {cf:checker_flags} : 
-  forall Σ {wfΣ : wf Σ.1} Γ t T (d : Σ ;;; Γ |- t : T),
-    forall Γl Γs Δ, 
-    is_strengthenable d #|Δ| #|Γs| -> 
-    Γ = Γl ,,, Γs ,,, lift_context #|Γs| 0 Δ ->
-    Σ ;;; Γl ,,, Δ |- rename (strengthen #|Δ| #|Γs|) t : rename (strengthen #|Δ| #|Γs|) T.
-Proof.
-  intros Σ wfΣ Γ t T d Γl. induction d; simpl.
-  - intros ? ? hn ->. admit.
-  - intros. admit.
-  - intros ? ?.
-    move/andP => [isd1 isd2]. intros ->.
-    rewrite /=. econstructor.
-    + eapply IHd1; eauto.
-    + specialize (IHd1 _ _ isd1 eq_refl).
-      pose proof (is_strengthenable_isLift _ isd1) as [[A' ->] _].
-      specialize (IHd2 _ (Δ,, vass na A') isd2).
-      forward IHd2. { now rewrite lift_context_snoc Nat.add_0_r. }
-      rewrite strengthen_lift.
-      rewrite shiftn_strengthen. { pose proof (is_strengthenable_isLift _ isd2). admit. }
-      apply IHd2.
-  - admit.
-  - admit.
-  - intros ? ?. move/and3P => [hd1 hd2 hd3]; intros ->.
-    specialize (IHd1 _ _ hd1 eq_refl).
-    specialize (IHd2 _ _ hd2 eq_refl).
-    specialize (IHd3 _ _ hd3 eq_refl).
-    eapply meta_conv.
-    + eapply type_App.
-    * simpl in IHd1. eapply IHd1; tea.
-    * simpl in IHd2. eapply IHd2.
-    * eapply IHd3.
-    + now rewrite rename_subst10.
-  - intros.
-    autorewrite with sigma.
-    admit.
-  - admit.
-  - admit.
-  - admit.
-  - admit.
-  - admit.
-  - admit.
-  - intros Γs Δ. move/andP=> [hd1 hd2]. intros ->.
-    specialize (IHd1 _ _ hd1 eq_refl).
-    specialize (IHd2 _ _ hd2 eq_refl).
-    epose proof (is_strengthenable_isLift _ hd1).
-    epose proof (is_strengthenable_isLift _ hd2).
-    eapply type_Cumul; eauto.
-    eapply cumul_renameP; eauto.
-    * apply (strengthen_urenaming Γl Γs Δ).
-    * destruct X. admit.
-Admitted.
-
-Lemma invert_cumul_prod_r {cf:checker_flags} Σ Γ C na A B :
-Σ ;;; Γ |- C <= tProd na A B ->
-∑ na' A' B', red Σ.1 Γ C (tProd na' A' B') *
-             eq_binder_annot na na' *
-             (Σ ;;; Γ |- A = A') *
-             (Σ ;;; (Γ ,, vass na A) |- B' <= B).
-Proof.
-Admitted.
-Lemma inversion_Prod {cf:checker_flags} Σ :
-    forall {Γ na A B T},
-      Σ ;;; Γ |- tProd na A B : T ->
-      ∑ s1 s2,
-        Σ ;;; Γ |- A : tSort s1 ×
-        Σ ;;; Γ ,, vass na A |- B : tSort s2 ×
-        Σ ;;; Γ |- tSort (Universe.sort_of_product s1 s2) <= T.
-  Proof.
-  Admitted.
-
-  Lemma type_reduction {cf} {Σ : global_env_ext} {wfΣ : wf Σ} {Γ t A B} : 
-    Σ ;;; Γ |- t : A -> red Σ Γ A B -> Σ ;;; Γ |- t : B.
-  Proof.
-  Admitted.
-
-Lemma noccur_iss {cf:checker_flags} : 
-  forall Σ {wfΣ : wf Σ.1} Γ t T (d : Σ ;;; Γ |- t : T),
-    forall Γl Γs Δ, 
-    Γ = Γl ,,, Γs ,,, lift_context #|Γs| 0 Δ ->
-    isLift #|Γs| #|Δ| t ->
-    ∑ T' (d' : Σ ;;; Γ |- t : T'), (is_strengthenable d' #|Δ| #|Γs|) × cumul Σ Γ T' T.
-Proof.
-  intros. induction d in Γs, Δ, X |- *.
-  - eexists; unshelve eexists; [econstructor; eauto|].
-    simpl. split; auto. 2:reflexivity. admit.
-  - admit.
-  - admit.
-  - admit.
-  - admit.
-  - destruct X as [[] ?]; noconf e.
-    specialize (IHd2 _ _ (isLift_lift _ _ _)) as [? [IHd2 [isd2 ?]]].
-    specialize (IHd3 _ _ (isLift_lift _ _ _)) as [? [IHd3 [isd3 ?]]].
-    pose proof (is_strengthenable_isLift _ isd2) as [? [? ->]].
-    eapply invert_cumul_prod_r in c as [? [? [? [[[? ?] ?] ?]]]].
-    exists (x3 {0 := (lift #|Γs| #|Δ| v)}).
-    unshelve eexists.
-    * epose proof (type_reduction IHd2 r).
-      econstructor.
-      2:eauto. 1:admit.
-      eapply type_Cumul'.
-      + eapply IHd3.
-      + admit.
-      + admit.
-    * simpl. admit.
-  - admit.
-  - admit.
-  - admit.
-  - admit.
-  - admit.
-  - admit.
-  - admit.
-  - specialize (IHd1 _ _ X) as [A' [dA' [? ?]]].
-    exists A', dA'. split; auto. admit.
-Admitted.
-    
-Lemma alli_mapi {A B} (f : nat -> A -> bool) (g : nat -> B -> A) n l : 
-  alli f n (mapi_rec g l n) = alli (fun i x => f i (g i x)) n l.
-Proof.
-  revert n; induction l => n; simpl; auto.
-  now rewrite IHl.
-Qed.
-
-Lemma alli_fold_context_prop f g ctx : 
-  alli f 0 (fold_context g ctx) =
-  alli (fun i x => f i (map_decl (g (Nat.pred #|ctx| - i)) x)) 0 ctx.
-Proof.
-  now rewrite fold_context_alt /mapi alli_mapi.
-Qed.
-
-Lemma test_decl_map_decl f g x : test_decl f (map_decl g x) = test_decl (f ∘ g) x.
-Proof.
-  rewrite /test_decl /map_decl /=.
-  f_equal. rewrite /foroptb. f_equal.
-  now rewrite option_map_two.
-Qed.
-
-Lemma all_free_vars_true t : all_free_vars xpredT t.
-Proof.
-Admitted.
-
-Lemma strengthen_thm {cf} : forall Σ {wfΣ : wf Σ.1} Γ t T (d : Σ ;;; Γ |- t : T),
-  forall Γl Γs Δ, 
-  Γ = Γl ,,, Γs ,,, lift_context #|Γs| 0 Δ ->
-  isLift #|Γs| #|Δ| t ->
-  isLift #|Γs| #|Δ| T ->
-  Σ ;;; Γl ,,, Δ |- rename (strengthen #|Δ| #|Γs|) t : rename (strengthen #|Δ| #|Γs|) T.
-Proof.
-  intros.
-  pose proof (noccur_iss _ _ _ _ d _ _ _ H X) as [T' [d' [isd cum]]].
-  pose proof (typing_rename_prop _ _ _ _ d' _ _ _ isd H).
-  eapply type_Cumul'; eauto.
-  * destruct X0 as [? ->].
-    rewrite strengthen_lift. admit.
-  * subst Γ. eapply cumul_renameP; eauto.
-    + eapply strengthen_urenaming.
-    + epose proof (is_strengthenable_isLift _ isd). admit.
-    + admit.
-    + unfold on_ctx_free_vars.
-      rewrite alli_app. apply/andP; split.
-      - rewrite /lift_context.
-        rewrite alli_fold_context_prop.
-        clear. eapply alli_Alli.
-        eapply forall_nth_error_Alli.
-        intros i x hnth. simpl.
-        eapply nth_error_Some_length in hnth.
-        rewrite {1}/nocc_betweenp. nat_compare_specs.
-        nat_compare_specs. simpl.
-        rewrite Nat.add_0_r.
-        rewrite /all_free_vars_decl.
-        rewrite test_decl_map_decl.
-        eapply (test_decl_impl (fun _ => true)).
-        { intros k _.
-          eapply all_free_vars_impl.
-          2:{ erewrite all_free_vars_lift. apply all_free_vars_true. } 
-          intros k'.
-          rewrite /strengthenP /nocc_betweenp /addnP.
-          repeat nat_compare_specs => /= //. }
-        destruct x as [na [?|] ? ]=> //.
-Admitted.
-
-(** For an unconditional renaming defined on all variables in the source context *)
-Lemma typing_rename_prop {cf:checker_flags} : env_prop
-  (fun Σ Γ t A =>
-    forall Γl Γs Δ, 
-    Γ = Γl ,,, Γs ,,, lift_context #|Γs| 0 Δ ->
-    isLift #|Γs| #|Δ| t ->
-    isLift #|Γs| #|Δ| A ->
-    Σ ;;; Γl ,,, Δ |- rename (strengthen #|Δ| #|Γs|) t : rename (strengthen #|Δ| #|Γs|) A)
-   (fun Σ Γ =>
-     forall Γl Γs Δ, 
-     Γ = Γl ,,, Γs ,,, lift_context #|Γs| 0 Δ ->
-     wf_local Σ (Γl ,,, Δ)).
-Proof.
-  apply typing_ind_env.
-
-  - intros Σ wfΣ Γ wfΓ HΓ.
-    intros Γl Γs Δ ->.
-    eapply wf_local_app. { clear HΓ. eapply wf_local_app_inv in wfΓ as [wfΓ _].
-      now apply wf_local_app_inv in wfΓ as []. }
-    apply All_local_env_over_simpl in HΓ.
-    apply All_local_env_app_inv in HΓ as [Hl HΔ].
-    clear Hl. apply All_local_env_fold in HΔ. clear -HΔ.
-    induction HΔ; constructor; firstorder eauto.
-    * red. exists x.
-      specialize (p _ _ _ eq_refl). rewrite Nat.add_0_r in p.
-      specialize (p (isLift_lift _ _ _) ((tSort x); eq_refl)).
-      simpl in p. now rewrite strengthen_lift in p.
-    * red. exists x.
-      specialize (p _ _ _ eq_refl). rewrite Nat.add_0_r in p.
-      specialize (p (isLift_lift _ _ _) ((tSort x); eq_refl)).
-      simpl in p. now rewrite strengthen_lift in p.
-    * red.
-      specialize (t1 _ _ _ eq_refl). rewrite Nat.add_0_r in t1.
-      specialize (t1 (isLift_lift _ _ _) (isLift_lift _ _ _)).
-      simpl in t1. now rewrite !strengthen_lift in t1.
-  
-  - intros Σ wfΣ Γ wfΓ n decl isdecl ihΓ Γl Γs Δ -> islt isla.
-    simpl in *. specialize (ihΓ _ _ _ eq_refl).
-    have hf := strengthen_urenaming Γl Γs Δ.
-    eapply hf in isdecl as h => //.
-    2:{ now apply isLift_rel in islt. }
-    destruct h as [decl' [isdecl' [? [h1 h2]]]].
-    rewrite lift0_rename rename_compose h1 -lift0_rename.
-    econstructor. all:auto.
-    rewrite /strengthen_context in isdecl'.
-    now rewrite strengthen_lift_ctx in isdecl'.
-
-  - intros Σ wfΣ Γ wfΓ l X H0 ? ? ? -> isl isl'.
-    simpl. constructor. all: eauto.
-
-  - intros Σ wfΣ Γ wfΓ na A B s1 s2 X hA ihA hB ihB ? ? ? -> isl isl'.
-    rewrite /=. econstructor.
-    + eapply ihA; eauto. all: admit.
-    + destruct isl. destruct x => //. simpl in e. noconf e.
-      specialize (ihB Γl Γs (Δ ,, vass na x1)).
-      forward ihB. { now rewrite lift_context_snoc Nat.add_0_r. }
-      specialize (ihB (isLift_lift _ _ _) (tSort _; eq_refl)).
-      rewrite strengthen_lift.
-      simpl in ihB. rewrite shiftn_strengthen. { admit. }
-      apply ihB.
-
-  - intros Σ wfΣ Γ wfΓ na A t s1 B X hA ihA ht iht P Δ f hf.
-    simpl. 
-     (* /andP [_ havB]. *)
-    simpl. econstructor.
-    + eapply ihA; eauto.
-    + eapply iht; eauto; simpl.
-      eapply renaming_extP. { now rewrite -(shiftnP_add 1). }
-      eapply renaming_vass. 2: eauto.
-      constructor.
-      * destruct hf as [hΔ hf]. auto.
-      * simpl. exists s1. eapply ihA; eauto.
-  - intros Σ wfΣ Γ wfΓ na b B t s1 A X hB ihB hb ihb ht iht P Δ f hf.
-    simpl. econstructor.
-    + eapply ihB; tea. 
-    + eapply ihb; tea.
-    + eapply iht; tea.
-      eapply renaming_extP. { now rewrite -(shiftnP_add 1). }
-      eapply renaming_vdef. 2: eauto.
-      constructor.
-      * destruct hf. assumption.
-      * simpl. eexists. eapply ihB; tea. 
-      * simpl. eapply ihb; tea.
-  - intros Σ wfΣ Γ wfΓ t na A B s u X hty ihty ht iht hu ihu P Δ f hf.
-    simpl. eapply meta_conv.
-    + eapply type_App.
-      * simpl in ihty. eapply ihty; tea.
-      * simpl in iht. eapply iht. eassumption.
-      * eapply ihu. eassumption.
-    + autorewrite with sigma. rewrite !subst1_inst. sigma.
-      eapply inst_ext => i.      
-      unfold subst_cons, ren, shiftn, subst_compose. simpl.
-      destruct i.
-      * simpl. reflexivity.
-      * simpl. replace (i - 0) with i by lia.
-        reflexivity.
-  - intros Σ wfΣ Γ wfΓ cst u decl X X0 isdecl hconst P Δ f hf.
-    simpl. eapply meta_conv.
-    + constructor. all: eauto. apply hf.
-    + rewrite rename_subst_instance_constr. f_equal.
-      rewrite rename_closed. 2: auto.
-      eapply declared_constant_closed_type. all: eauto.
-  - intros Σ wfΣ Γ wfΓ ind u mdecl idecl isdecl X X0 hconst P Δ σ hf.
-    simpl. eapply meta_conv.
-    + econstructor. all: eauto. apply hf.
-    + rewrite rename_subst_instance_constr. f_equal.
-      rewrite rename_closed. 2: auto.
-      eapply declared_inductive_closed_type. all: eauto.
-  - intros Σ wfΣ Γ wfΓ ind i u mdecl idecl cdecl isdecl X X0 hconst P Δ f hf.
-    simpl. eapply meta_conv.
-    + econstructor. all: eauto. apply hf. 
-    + rewrite rename_closed. 2: reflexivity.
-      eapply declared_constructor_closed_type. all: eauto.
-  - intros Σ wfΣ Γ wfΓ ci p c brs indices ps mdecl idecl isdecl HΣ.
-    intros IHΔ ci_npar predctx wfp Hpret IHpret IHpredctx isallowed.
-    intros Hc IHc iscof ptm wfbrs Hbrs P Δ f Hf.
-    simpl.
-    rewrite rename_mkApps.
-    rewrite map_app. simpl.
-    rewrite /ptm. rewrite rename_it_mkLambda_or_LetIn.
-    relativize #|predctx|.
-    * erewrite rename_predicate_preturn.
-      rewrite /predctx.
-      rewrite (rename_case_predicate_context isdecl wfp).
-      eapply type_Case; eauto.
-      + now eapply rename_wf_predicate.
-      + eapply IHpret.
-        rewrite -rename_case_predicate_context //.
-        split.
-        ++ apply All_local_env_app_inv in IHpredctx as [].
-          eapply wf_local_app_renaming; eauto. apply a0.
-        ++ rewrite /predctx.
-           rewrite -(case_predicate_context_length (ci:=ci) wfp).
-           eapply urenaming_ext.
-           { len. now rewrite -shiftnP_add. }
-           { reflexivity. }
-          eapply urenaming_context. apply Hf.
-      + simpl. unfold id.
-        specialize (IHc _ _ _ Hf).
-        now rewrite rename_mkApps map_app in IHc.
-      + now eapply rename_wf_branches.
-      + eapply Forall2_All2 in wfbrs.
-        eapply All2i_All2_mix_left in Hbrs; eauto.
-        eapply All2i_nth_hyp in Hbrs.
-        eapply All2i_map_right, (All2i_impl Hbrs) => i cdecl br.
-        set (brctxty := case_branch_type _ _ _ _ _ _ _ _).
-        move=> [Hnth [wfbr [[Hbr Hbrctx] [IHbr [Hbty IHbty]]]]].
-        rewrite -(rename_closed_constructor_body mdecl cdecl f).
-        { eapply (declared_constructor_closed (c:=(ci.(ci_ind),i))); eauto.
-          split; eauto. }
-        rewrite rename_case_branch_type //.
-        rewrite -/brctxty. intros brctx'.
-        assert (wf_local Σ (Δ,,, brctx'.1)).
-        { rewrite /brctx'. cbn.
-          apply All_local_env_app_inv in Hbrctx as [].
-          eapply wf_local_app_renaming; tea. apply a0. }
-        repeat split.
-        ++ eapply IHbr. 
-          split => //.
-          rewrite /brctx' /brctxty; cbn.
-          rewrite (wf_branch_length wfbr).
-          erewrite <- case_branch_type_length; eauto.
-          eapply urenaming_ext.
-          { now rewrite app_context_length -shiftnP_add. }
-          { reflexivity. }
-          eapply urenaming_context, Hf.
-        ++ eapply IHbty. split=> //.
-          rewrite /brctx'; cbn.
-          rewrite (wf_branch_length wfbr).
-          erewrite <- case_branch_type_length; eauto.
-          eapply urenaming_ext.
-          { now rewrite app_context_length -shiftnP_add. }
-          { reflexivity. }
-          eapply urenaming_context, Hf.
-    * rewrite /predctx case_predicate_context_length //.
-  - intros Σ wfΣ Γ wfΓ p c u mdecl idecl pdecl isdecl args X X0 hc ihc e ty
-           P Δ f hf.
-    simpl. eapply meta_conv.
-    + econstructor.
-      * eassumption.
-      * eapply meta_conv.
-        -- eapply ihc; tea.
-        -- rewrite rename_mkApps. simpl. reflexivity.
-      * rewrite map_length. assumption.
-    + rewrite rename_subst0. simpl. rewrite map_rev. f_equal.
-      rewrite rename_subst_instance_constr. f_equal.
-      rewrite rename_closedn. 2: reflexivity.
-      eapply declared_projection_closed_type in isdecl.
-      rewrite List.rev_length. rewrite e. assumption.
-
-  - intros Σ wfΣ Γ wfΓ mfix n decl types H1 hdecl X ihmfixt ihmfixb wffix P Δ f hf.
-    apply All_local_env_app_inv in X as [_ X].
-    eapply wf_local_app_renaming in X; tea.
-    simpl. eapply meta_conv.
-    + eapply type_Fix.
-      * eapply fix_guard_rename; eauto.
-      * rewrite nth_error_map. rewrite hdecl. simpl. reflexivity.
-      * apply hf.
-      * apply All_map, (All_impl ihmfixt).
-        intros x [s [Hs IHs]].
-        exists s. now eapply IHs.
-      * apply All_map, (All_impl ihmfixb).
-        intros x [Hb IHb].
-        destruct x as [na ty bo rarg]. simpl in *.
-        rewrite rename_fix_context.
-        eapply meta_conv.
-        ++ apply (IHb P (Δ ,,, rename_context f types) (shiftn #|mfix| f)).
-          split; auto. subst types. rewrite -(fix_context_length mfix).
-          eapply urenaming_ext.
-          { now rewrite app_context_length -shiftnP_add. }
-          { reflexivity. }
-          apply urenaming_context; auto. apply hf.
-        ++ len; now sigma.
-      * now eapply rename_wf_fixpoint.
-    + reflexivity.
-
-  - intros Σ wfΣ Γ wfΓ mfix n decl types guard hdecl X ihmfixt ihmfixb wfcofix P Δ f hf.
-    apply All_local_env_app_inv in X as [_ X].
-    eapply wf_local_app_renaming in X; eauto.
-    simpl. eapply meta_conv.
-    + eapply type_CoFix; auto.
-      * eapply cofix_guard_rename; eauto.
-      * rewrite nth_error_map. rewrite hdecl. simpl. reflexivity.
-      * apply hf.
-      * apply All_map, (All_impl ihmfixt).
-        intros x [s [Hs IHs]].
-        exists s. now eapply IHs.
-      * apply All_map, (All_impl ihmfixb).
-        intros x [Hb IHb].
-        destruct x as [na ty bo rarg]. simpl in *.
-        rewrite rename_fix_context.
-        eapply meta_conv.
-        ++ apply (IHb P (Δ ,,, rename_context f types) (shiftn #|mfix| f)).
-            split; auto. subst types. rewrite -(fix_context_length mfix).
-            eapply urenaming_ext.
-            { now rewrite app_context_length -shiftnP_add. }
-            { reflexivity. }
-            apply urenaming_context; auto. apply hf.
-        ++ len. now sigma.
-      * now eapply rename_wf_cofixpoint.
-    + reflexivity.
-
-  - intros Σ wfΣ Γ wfΓ t A B X hwf ht iht htB ihB cum P Δ f hf.
-    eapply type_Cumul.
-    + eapply iht; tea.
-    + eapply ihB; tea.
-    + eapply cumul_renameP. all: try eassumption.
-      * apply hf.
-      * pose proof (type_closed _ ht).
-        now eapply closedn_all_free_vars in H.
-      * pose proof (subject_closed _ htB).
-        now eapply closedn_all_free_vars in H.
-      * pose proof (closed_ctx_all_free_vars P _ (closed_wf_local _ (typing_wf_local ht))).
-        rewrite -{2}(app_context_nil_l Γ).
-        eapply on_ctx_free_vars_extend => //.
-Qed.
-
-
-Lemma strengthening_wf_local {cf: checker_flags} {Σ : global_env_ext} {wfΣ : wf Σ} {Γ Γ' Γ''} :
-  wf_local Σ (Γ ,,, Γ' ,,, lift_context #|Γ'| 0 Γ'') ->
-  wf_local Σ (Γ ,,, Γ'').
-Proof.
-  intros wfΓ'.
-  pose proof (env_prop_wf_local _ _ typing_rename_prop _ wfΣ _ wfΓ'). simpl in X.
-  eapply All_local_env_app_inv in X as [XΓ XΓ'].
-  apply wf_local_app_inv in wfΓ' as [wfΓ wfΓ''].
-  apply wf_local_app_inv in wfΓ as [wfΓ wfΓ'].
-  apply wf_local_app => //.
-  apply All_local_env_fold in XΓ'.
-  eapply (All_local_env_impl_ind XΓ').
-  intros Δ t [T|] IH; unfold lift_typing; simpl.
-  - rewrite -/(lift_context #|Γ'| 0 Δ).
-    intros Hf. red.
-    rewrite Nat.add_0_r in Hf. rewrite !lift_rename in Hf.
-    specialize (Hf (nocc_betweenp #|Δ| #|Γ'|) (Γ ,,, Δ) (strengthen #|Δ| #|Γ'|)).
-    forward Hf.
-    * split.
-      + apply wf_local_app; auto.
-      + len. rewrite /shiftnP.
-        epose proof (strengthen_urenaming Γ Γ' Δ). simpl in X.
-        rewrite /strengthen_context in X.
-        rewrite /PCUICRename.shiftnP.
-
-    eapply (Hf (fun x => true)).
-    split.
-    + apply wf_local_app; auto.
-      apply All_local_env_fold in IH. apply IH.
-    + apply (weakening_renaming _ Γ Δ Γ'').
-  - intros [s Hs]; exists s. red.
-    rewrite -/(lift_context #|Γ''| 0 Δ).
-    rewrite Nat.add_0_r !lift_rename. 
-    apply (Hs (fun _ => true)).
-    split.
-    + apply wf_local_app; auto.
-      apply All_local_env_fold in IH. apply IH.
-    + apply (weakening_renaming _ Γ Δ Γ'').
-Qed.
-
-Lemma exchange_wf_local {cf: checker_flags} {Σ : global_env_ext} {wfΣ : wf Σ} {Γ Γl Γr Δ} :
-  noccur_between_ctx 0 #|Γl| Γr ->
-  wf_local Σ (Γ ,,, Γl ,,, Γr ,,, Δ) ->
-  wf_local Σ (exchange_contexts Γ Γl Γr Δ).
-Proof.
-  intros nocc wf.
-  pose proof (env_prop_wf_local _ _ typing_rename_prop _ wfΣ _ wf).
-  simpl in X. rewrite /exchange_contexts.
-  eapply All_local_env_app_inv in X as [XΓ XΓ'].
-  apply wf_local_app_ind => //.
-  - rewrite rename_context_lift_context /strengthen /=.
-    eapply weakening_wf_local_eq; eauto with wf.
-    * admit.
-    * now len.
-  - intros wfstr.
-    apply All_local_env_fold.
-    eapply (All_local_env_impl_ind XΓ').
-    intros Δ' t [T|] IH; unfold lift_typing; simpl.
-    * intros Hf. red.
-      eapply meta_conv_all. 2: reflexivity.
-      2-3:now rewrite shiftn_exchange_renaming.
-      apply Hf. split.
-      + apply wf_local_app; auto.
-        apply All_local_env_fold in IH. apply IH.
-      + setoid_rewrite shiftn_exchange_renaming. apply exchange_urenaming.
-    - intros [s Hs]; exists s. red.
-      rewrite -/(lift_context #|Γ''| 0 Δ).
-      rewrite Nat.add_0_r !lift_rename. apply Hs.
-      split.
-      + apply wf_local_app; auto.
-        apply All_local_env_fold in IH. apply IH.
-      + apply (weakening_renaming Γ Δ Γ'').
-Qed.
-
-Lemma exchange_typing `{cf : checker_flags} {Σ : global_env_ext} {wfΣ : wf Σ} {Γ Γ' Γ''} {t T} :
-  wf_local Σ (Γ ,,, Γ'') ->
-  Σ ;;; Γ ,,, Γ' |- t : T ->
-  Σ ;;; Γ ,,, Γ'' ,,, lift_context #|Γ''| 0 Γ' |- lift #|Γ''| #|Γ'| t : lift #|Γ''| #|Γ'| T.
-Proof.
-  intros wfext Ht.
-  rewrite !lift_rename.
-  eapply (env_prop_typing _ _ typing_rename_prop); eauto.
-  split.
-  - eapply weakening_wf_local; eauto with pcuic.
-  - now apply weakening_renaming.
-Qed.
-
-
-
-
 Lemma decompose_prod_assum_ctx ctx t : decompose_prod_assum ctx t =
   let (ctx', t') := decompose_prod_assum [] t in
   (ctx ,,, ctx', t').
@@ -1438,7 +279,6 @@ Proof.
     destruct (decompose_prod_assum [] t3). simpl.
     unfold snoc. now rewrite app_context_assoc.
 Qed.
-
 
 Lemma smash_context_lift Δ k n Γ :
   smash_context (lift_context n (k + #|Γ|) Δ) (lift_context n k Γ) =
@@ -1507,304 +347,31 @@ Lemma lift_declared_constant `{checker_flags} Σ cst decl n k :
   declared_constant Σ cst decl ->
   decl = map_constant_body (lift n k) decl.
 Proof.
-  unfold declared_constant.
-  intros.
-  eapply lookup_on_global_env in H0; eauto.
-  destruct H0 as [Σ' [wfΣ' decl']].
-  red in decl'. red in decl'.
-  destruct decl. simpl in *. destruct cst_body.
-  - unfold map_constant_body. simpl.
-    pose proof decl' as declty.
-    apply typecheck_closed in declty; eauto.
-    + destruct declty as [declty Hcl].
-      rewrite -> andb_and in Hcl. destruct Hcl as [clb clty].
-      pose proof (closed_upwards k clb).
-      pose proof (closed_upwards k clty).
-      simpl in *. forward H0 by lia. forward H1 by lia.
-      apply (lift_closed n k) in H0.
-      apply (lift_closed n k) in H1. rewrite H0 H1. reflexivity.
-
-  - red in decl'.
-    destruct decl'.
-    apply subject_closed in t; auto.
-    eapply closed_upwards in t; simpl.
-    * apply (lift_closed n k) in t. unfold map_constant_body. simpl.
-      rewrite t. reflexivity.
-    * lia.
+  intros wf declc.
+  rewrite /map_constant_body; destruct decl; simpl; f_equal; rewrite ?lift_rename.
+  - eapply declared_constant_closed_type in declc; eauto.
+    now rewrite rename_closed.
+  - destruct cst_body eqn:cb => /= //.
+    f_equal.
+    eapply declared_constant_closed_body in declc; simpl; eauto.
+    now rewrite lift_rename rename_closed.
 Qed.
 
 Definition lift_mutual_inductive_body n k m :=
   map_mutual_inductive_body (fun k' => lift n (k' + k)) m.
-
-Lemma lift_wf_local `{checker_flags} Σ Γ n k :
-  wf Σ.1 ->
-  wf_local Σ Γ ->
-  lift_context n k Γ = Γ.
-Proof.
-  intros wfΣ.
-  induction 1; auto; unfold lift_context, snoc; rewrite fold_context_snoc0; auto; unfold snoc;
-    f_equal; auto; unfold map_decl; simpl.
-  - destruct t0 as [s Hs]. unfold vass. f_equal.
-    eapply typed_liftn; eauto. lia.
-  - red in t0. destruct t0. unfold vdef. f_equal.
-    + f_equal. eapply typed_liftn; eauto. lia.
-    + eapply typed_liftn in t0 as [Ht HT]; eauto. lia.
-Qed.
-
-Lemma lift_declared_minductive `{checker_flags} {Σ : global_env} cst decl n k :
-  wf Σ ->
-  declared_minductive Σ cst decl ->
-  lift_mutual_inductive_body n k decl = decl.
-Proof.
-  intros wfΣ Hdecl.
-  pose proof (on_declared_minductive wfΣ Hdecl). apply onNpars in X.
-  apply (declared_inductive_closed (Σ:=(empty_ext Σ))) in Hdecl; auto.
-  move: Hdecl.
-  rewrite /closed_inductive_decl /lift_mutual_inductive_body.
-  destruct decl; simpl.
-  move/andb_and => [clpar clbodies]. f_equal.
-  - now rewrite [fold_context _ _]closed_ctx_lift.
-  - eapply forallb_All in clbodies.
-    eapply Alli_mapi_id.
-    * eapply (All_Alli clbodies). intros; eauto.
-      intros. eapply H0.
-    * simpl; intros.
-      move: H0. rewrite /closed_inductive_body.
-      destruct x; simpl. move=> /andb_and[/andb_and [ci ct] cp].
-      f_equal.
-      + rewrite lift_closed; eauto.
-        eapply closed_upwards; eauto; lia.
-      + eapply All_map_id. eapply forallb_All in ct.
-        eapply (All_impl ct). intros x.
-        destruct x as [[id ty] arg]; unfold on_pi2; intros c; simpl; repeat f_equal.
-        apply lift_closed. unfold cstr_type in c; simpl in c.
-        eapply closed_upwards; eauto; lia.
-      + simpl in X. rewrite -X in cp.
-        eapply forallb_All in cp. eapply All_map_id; eauto.
-        eapply (All_impl cp); intuition auto.
-        destruct x; unfold on_snd; simpl; f_equal.
-        apply lift_closed. rewrite context_assumptions_fold.
-        eapply closed_upwards; eauto; lia.
-Qed.
-
-Lemma lift_declared_inductive `{checker_flags} ind Σ mdecl idecl n k :
-  wf Σ ->
-  declared_inductive Σ ind mdecl idecl ->
-  map_one_inductive_body (context_assumptions mdecl.(ind_params))
-                         (length (arities_context mdecl.(ind_bodies))) (fun k' => lift n (k' + k))
-                         (inductive_ind ind) idecl = idecl.
-Proof.
-  unfold declared_inductive. intros wfΣ [Hmdecl Hidecl].
-  eapply (lift_declared_minductive _ _ n k) in Hmdecl. 2: auto.
-  unfold lift_mutual_inductive_body in Hmdecl.
-  destruct mdecl. simpl in *.
-  injection Hmdecl. intros Heq.
-  clear Hmdecl.
-  pose proof Hidecl as Hidecl'.
-  rewrite <- Heq in Hidecl'.
-  rewrite nth_error_mapi in Hidecl'.
-  clear Heq.
-  unfold option_map in Hidecl'. rewrite Hidecl in Hidecl'.
-  congruence.
-Qed.
-
-Lemma subst0_inds_lift ind u mdecl n k t :
-  (subst0 (inds (inductive_mind ind) u (ind_bodies mdecl))
-          (lift n (#|arities_context (ind_bodies mdecl)| + k) t)) =
-  lift n k (subst0 (inds (inductive_mind ind) u (ind_bodies mdecl)) t).
-Proof.
-  rewrite (distr_lift_subst_rec _ _ n 0 k). simpl.
-  unfold arities_context. rewrite rev_map_length inds_length.
-  f_equal. generalize (ind_bodies mdecl).
-  clear. intros.
-  induction l; unfold inds; simpl; auto. f_equal. auto.
-Qed.
-
-Lemma lift_declared_constructor `{checker_flags} Σ c u mdecl idecl cdecl n k :
-  wf Σ ->
-  declared_constructor Σ c mdecl idecl cdecl ->
-  lift n k (type_of_constructor mdecl cdecl c u) = (type_of_constructor mdecl cdecl c u).
-Proof.
-  unfold declared_constructor. destruct c as [i ci]. intros wfΣ [Hidecl Hcdecl].
-  eapply (lift_declared_inductive _ _ _ _ n k) in Hidecl; eauto.
-  unfold type_of_constructor. destruct cdecl as [[id t'] arity].
-  destruct idecl; simpl in *.
-  injection Hidecl.
-  intros.
-  pose Hcdecl as Hcdecl'.
-  rewrite <- H1 in Hcdecl'.
-  rewrite nth_error_map in Hcdecl'. rewrite Hcdecl in Hcdecl'.
-  simpl in Hcdecl'. injection Hcdecl'.
-  intros.
-  rewrite <- H3 at 2.
-  rewrite <- lift_subst_instance_constr.
-  now rewrite subst0_inds_lift.
-Qed.
-
-Lemma lift_declared_projection `{checker_flags} Σ c mdecl idecl pdecl n k :
-  wf Σ ->
-  declared_projection Σ c mdecl idecl pdecl ->
-  on_snd (lift n (S (ind_npars mdecl + k))) pdecl = pdecl.
-Proof.
-  intros.
-  eapply (declared_projection_closed (Σ:=empty_ext Σ)) in H0; auto.
-  unfold on_snd. simpl.
-  rewrite lift_closed.
-  - eapply closed_upwards; eauto; try lia.
-  - destruct pdecl; reflexivity.
-Qed.
 
 Lemma lift_fix_context:
   forall (mfix : list (def term)) (n k : nat),
     fix_context (map (map_def (lift n k) (lift n (#|mfix| + k))) mfix) = lift_context n k (fix_context mfix).
 Proof.
   intros mfix n k. unfold fix_context.
-  rewrite map_vass_map_def rev_mapi.
+  rewrite PCUICLiftSubst.map_vass_map_def rev_mapi.
   fold (fix_context mfix).
   rewrite (lift_context_alt n k (fix_context mfix)).
   unfold lift_decl. now rewrite mapi_length fix_context_length.
 Qed.
 
 Hint Rewrite <- lift_fix_context : lift.
-
-Lemma All_local_env_lift `{checker_flags}
-      (P Q : context -> term -> option term -> Type) c n k :
-  All_local_env Q c ->
-  (forall Γ t T,
-      Q Γ t T ->
-      P (lift_context n k Γ) (lift n (#|Γ| + k) t)
-        (option_map (lift n (#|Γ| + k)) T)
-  ) ->
-  All_local_env P (lift_context n k c).
-Proof.
-  intros Hq Hf.
-  induction Hq in |- *; try econstructor; eauto;
-    simpl; rewrite lift_context_snoc; econstructor; eauto.
-  - simpl. eapply (Hf _ _ None). eauto.
-  - simpl. eapply (Hf _ _ None). eauto.
-  - simpl. eapply (Hf _ _ (Some t)). eauto.
-Qed.
-
-Lemma lift_destArity ctx t n k :
-  destArity (lift_context n k ctx) (lift n (#|ctx| + k) t) =
-        match destArity ctx t with
-        | Some (args, s) => Some (lift_context n k args, s)
-        | None => None
-        end.
-Proof.
-  revert ctx.
-  induction t in n, k |- * using term_forall_list_ind; intros ctx; simpl; trivial.
-  - move: (IHt2 n k (ctx,, vass n0 t1)).
-    now rewrite lift_context_snoc /= /lift_decl /map_decl /vass /= => ->.
-  - move: (IHt3 n k (ctx,, vdef n0 t1 t2)).
-    now rewrite lift_context_snoc /= /lift_decl /map_decl /vass /= => ->.
-Qed.
-
-(* Lemma lift_strip_outer_cast n k t : lift n k (strip_outer_cast t) = strip_outer_cast (lift n k t). *)
-(* Proof. *)
-(*   induction t; simpl; try reflexivity. *)
-(*   destruct Nat.leb; reflexivity. *)
-(*   now rewrite IHt1. *)
-(* Qed. *)
-
-Definition on_pair {A B C D} (f : A -> B) (g : C -> D) (x : A * C) :=
-  (f (fst x), g (snd x)).
-
-Lemma lift_instantiate_params_subst n k params args s t :
-  instantiate_params_subst (mapi_rec (fun k' decl => lift_decl n (k' + k) decl) params #|s|)
-                           (map (lift n k) args) (map (lift n k) s) (lift n (#|s| + k) t) =
-  option_map (on_pair (map (lift n k)) (lift n (#|s| + k + #|params|))) (instantiate_params_subst params args s t).
-Proof.
-  induction params in args, t, n, k, s |- *.
-  - destruct args; simpl; rewrite ?Nat.add_0_r; reflexivity.
-  - simpl. simpl. (* rewrite <- lift_strip_outer_cast. generalize (strip_outer_cast t). *)
-    (* clear t; intros t. *)
-    destruct a as [na [body|] ty]; simpl; try congruence.
-    + destruct t; simpl; try congruence.
-      specialize (IHparams n k args (subst0 s body :: s) t3).
-      rewrite <- Nat.add_succ_r. simpl in IHparams.
-      rewrite Nat.add_succ_r.
-      replace (#|s| + k + S #|params|) with (S (#|s| + k + #|params|)) by lia.
-      rewrite <- IHparams.
-      rewrite distr_lift_subst. reflexivity.
-    + destruct t; simpl; try congruence.
-      destruct args; simpl; try congruence.
-      specialize (IHparams n k args (t :: s) t2). simpl in IHparams.
-      replace (#|s| + k + S #|params|) with (S (#|s| + k + #|params|)) by lia.
-      rewrite <- IHparams. auto.
-Qed.
-
-Lemma instantiate_params_subst_length params args s t ctx t' :
-  instantiate_params_subst params args s t = Some (ctx, t') ->
-  #|ctx| = #|s| + #|params|.
-Proof.
-  induction params in args, s, t, ctx, t' |- * ;
-  destruct args; simpl; auto; try congruence.
-  - rewrite Nat.add_0_r. congruence.
-  - destruct decl_body.
-    + simpl.
-      destruct t; simpl; try congruence.
-      intros. erewrite IHparams; eauto. simpl. lia.
-    + destruct t; simpl; try congruence.
-  - destruct decl_body.
-    + simpl.
-      destruct t; simpl; try congruence.
-      intros. erewrite IHparams; eauto. simpl. lia.
-    + destruct t; simpl; try congruence.
-      intros. erewrite IHparams; eauto. simpl. lia.
-Qed.
-
-Lemma closed_tele_lift n k ctx :
-  closed_ctx ctx ->
-  mapi (fun (k' : nat) (decl : context_decl) => lift_decl n (k' + k) decl) (List.rev ctx) = List.rev ctx.
-Proof.
-  rewrite /closedn_ctx /mapi. simpl. generalize 0.
-  induction ctx using rev_ind.
-  1: move=> //.
-  move=> n0.
-  rewrite /closedn_ctx !rev_app_distr /id /=.
-  move/andb_and => [closedx Hctx].
-  rewrite lift_decl_closed.
-  - rewrite (@closed_decl_upwards n0) //; try lia.
-  - f_equal. now rewrite IHctx.
-Qed.
-
-Lemma lift_instantiate_params n k params args t :
-  closed_ctx params ->
-  option_map (lift n k) (instantiate_params params args t) =
-  instantiate_params params (map (lift n k) args) (lift n k t).
-Proof.
-  unfold instantiate_params.
-  move/(closed_tele_lift n k params)=> Heq.
-  rewrite -{2}Heq.
-  specialize (lift_instantiate_params_subst n k (List.rev params) args [] t).
-  move=> /= Heq'; rewrite Heq'.
-  case E: (instantiate_params_subst (List.rev params) args)=> [[l' t']|] /= //.
-  rewrite distr_lift_subst.
-  move/instantiate_params_subst_length: E => -> /=.  do 3 f_equal. lia.
-Qed.
-Hint Rewrite lift_instantiate_params : lift.
-
-Lemma lift_decompose_prod_assum_rec ctx t n k :
-  (let (ctx', t') := decompose_prod_assum ctx t in
-  (lift_context n k ctx', lift n (length ctx' + k) t')) =
-  decompose_prod_assum (lift_context n k ctx) (lift n (length ctx + k) t).
-Proof.
-  induction t in n, k, ctx |- *; simpl;
-    try rewrite -> Nat.sub_diag, Nat.add_0_r; try (eauto; congruence).
-  - specialize (IHt2 (ctx ,, vass na t1) n k).
-    destruct decompose_prod_assum. rewrite IHt2. simpl.
-    rewrite lift_context_snoc. reflexivity.
-  - specialize (IHt3 (ctx ,, vdef na t1 t2) n k).
-    destruct decompose_prod_assum. rewrite IHt3. simpl.
-    rewrite lift_context_snoc. reflexivity.
-Qed.
-
-Lemma lift_decompose_prod_assum t n k :
-  (let (ctx', t') := decompose_prod_assum [] t in
-  (lift_context n k ctx', lift n (length ctx' + k) t')) =
-  decompose_prod_assum [] (lift n k t).
-Proof. apply lift_decompose_prod_assum_rec. Qed.
 
 Lemma lift_it_mkProd_or_LetIn n k ctx t :
   lift n k (it_mkProd_or_LetIn ctx t) =
@@ -1817,19 +384,6 @@ Proof.
   now destruct a as [na [b|] ty].
 Qed.
 Hint Rewrite lift_it_mkProd_or_LetIn : lift.
-
-Lemma to_extended_list_lift n k c :
-  to_extended_list (lift_context n k c) = to_extended_list c.
-Proof.
-  unfold to_extended_list, to_extended_list_k. generalize 0.
-  unf_term. generalize (@nil term) at 1 2.
-  induction c in n, k |- *; simpl; intros. 1: reflexivity.
-  rewrite -> lift_context_snoc0. unfold snoc. simpl.
-  destruct a. destruct decl_body.
-  - unfold lift_decl, map_decl. simpl.
-    now rewrite -> IHc.
-  - simpl. apply IHc.
-Qed.
 
 Lemma to_extended_list_map_lift:
   forall (n k : nat) (c : context), to_extended_list c = map (lift n (#|c| + k)) (to_extended_list c).
@@ -1849,88 +403,10 @@ Lemma weakening_red1 `{CF:checker_flags} Σ Γ Γ' Γ'' M N :
   red1 Σ (Γ ,,, Γ'' ,,, lift_context #|Γ''| 0 Γ') (lift #|Γ''| #|Γ'| M) (lift #|Γ''| #|Γ'| N).
 Proof.
   intros wfΣ H.
-  remember (Γ ,,, Γ') as Γ0. revert Γ Γ' Γ'' HeqΓ0.
-  induction H using red1_ind_all in |- *; intros Γ0 Γ' Γ'' HeqΓ0; try subst Γ; simpl;
-    autorewrite with lift;
-    try solve [  econstructor; eauto with pcuic ].
-
-  - elim (leb_spec_Set); intros Hn.
-    + rewrite -> simpl_lift; try lia. rewrite -> Nat.add_succ_r.
-      econstructor; eauto.
-      erewrite (weaken_nth_error_ge Hn) in H. eauto.
-
-    + rewrite <- lift_simpl by easy.
-      econstructor.
-      rewrite -> (weaken_nth_error_lt Hn).
-      now unfold lift_decl; rewrite -> option_map_decl_body_map_decl, H.
-
-  - econstructor; eauto with pcuic.
-    rewrite H0. f_equal.
-    eapply (lookup_on_global_env _ _ _ _ wfΣ) in H.
-    destruct H as [Σ' [wfΣ' decl']].
-    red in decl'. red in decl'.
-    rewrite -> H0 in decl'.
-    apply typecheck_closed in decl'; eauto.
-    destruct decl'.
-    rewrite -> andb_and in i. destruct i as [Hclosed _].
-    simpl in Hclosed.
-    pose proof (closed_upwards #|Γ'| Hclosed).
-    forward H by lia.
-    apply (lift_closed #|Γ''| #|Γ'|) in H. auto.
-
-  - simpl. constructor.
-    now rewrite -> nth_error_map, H.
-
-  - constructor.
-    specialize (IHred1 Γ0 (Γ' ,, vass na N) Γ'' eq_refl).
-    rewrite -> lift_context_snoc, Nat.add_0_r in IHred1. apply IHred1.
-
-  - constructor.
-    specialize (IHred1 Γ0 (Γ' ,, vdef na b t) Γ'' eq_refl).
-    rewrite -> lift_context_snoc, Nat.add_0_r in IHred1. apply IHred1.
-
-  - constructor.
-    induction X; constructor; auto.
-    intuition; eauto.
-
-  - constructor.
-    specialize (IHred1 Γ0 (Γ' ,, vass na M1) Γ'' eq_refl).
-    rewrite -> lift_context_snoc, Nat.add_0_r in IHred1. apply IHred1.
-
-  - constructor.
-    induction X; constructor; auto.
-    intuition; eauto.
-
-  - constructor.
-    rewrite -> (OnOne2_length X). generalize (#|mfix1|).
-    induction X; simpl; constructor; simpl; intuition eauto.
-    congruence.
-
-  - apply fix_red_body. rewrite !lift_fix_context.
-    rewrite <- (OnOne2_length X).
-    eapply OnOne2_map. unfold on_Trel; solve_all. 2: congruence.
-    specialize (b0 Γ0 (Γ' ,,, fix_context mfix0)).
-    rewrite app_context_assoc in b0. specialize (b0 Γ'' eq_refl).
-    rewrite -> app_context_length, fix_context_length in *.
-    rewrite -> lift_context_app in *.
-    rewrite -> app_context_assoc, Nat.add_0_r in *.
-    auto.
-
-  - constructor.
-    rewrite -> (OnOne2_length X). generalize (#|mfix1|).
-    induction X; simpl; constructor; intuition eauto.
-    + simpl; auto.
-    + simpl; congruence.
-
-  - apply cofix_red_body. rewrite !lift_fix_context.
-    rewrite <- (OnOne2_length X).
-    eapply OnOne2_map. unfold on_Trel; solve_all. 2: congruence.
-    specialize (b0 Γ0 (Γ' ,,, fix_context mfix0)).
-    rewrite app_context_assoc in b0. specialize (b0 Γ'' eq_refl).
-    rewrite -> app_context_length, fix_context_length in *.
-    rewrite -> lift_context_app in *.
-    rewrite -> app_context_assoc, Nat.add_0_r in *.
-    auto.
+  rewrite !lift_rename.
+  eapply red1_rename; eauto.
+  - eapply weakening_renaming.
+  - eapply on_free_vars_true. 
 Qed.
 
 Lemma weakening_red `{CF:checker_flags} Σ Γ Γ' Γ'' M N :
@@ -1984,19 +460,31 @@ Fixpoint lift_stack n k π :=
       let mfix1' := List.map (map_def (lift n k') (lift n k'')) mfix1 in
       let mfix2' := List.map (map_def (lift n k') (lift n k'')) mfix2 in
       CoFix_mfix_bd na (lift n k' ty) ra mfix1' mfix2' idx (lift_stack n k π)
-  | Case_p indn c brs π =>
+  | Case_pars ci pars1 pars2 puinst pctx p c brs π =>
       let k' := #|stack_context π| + k in
-      let brs' := List.map (on_snd (lift n k')) brs in
-      Case_p indn (lift n k' c) brs' (lift_stack n k π)
-  | Case indn pred brs π =>
+      let brs' := map_branches_k (lift n) k' brs in
+      Case_pars ci 
+        (List.map (lift n k') pars1)
+        (List.map (lift n k') pars2) 
+        puinst pctx
+        (lift n (#|pctx| + k') p)
+        (lift n k' c) brs' (lift_stack n k π)
+  | Case_p ci pars puinst pctx c brs π =>
       let k' := #|stack_context π| + k in
-      let brs' := List.map (on_snd (lift n k')) brs in
-      Case indn (lift n k' pred) brs' (lift_stack n k π)
-  | Case_brs indn pred c m brs1 brs2 π =>
+      let brs' := map_branches_k (lift n) k' brs in
+      Case_p ci (List.map (lift n k') pars) puinst (lift_context n k' pctx) 
+        (lift n k' c) brs' (lift_stack n k π)
+  | Case ci pred brs π =>
       let k' := #|stack_context π| + k in
-      let brs1' := List.map (on_snd (lift n k')) brs1 in
-      let brs2' := List.map (on_snd (lift n k')) brs2 in
-      Case_brs indn (lift n k' pred) (lift n k' c) m brs1' brs2' (lift_stack n k π)
+      let pred' := map_predicate id (lift n k') (lift n (#|pred.(pcontext)| + k')) pred in
+      let brs' := map_branches_k (lift n) k' brs in
+      Case ci pred' brs' (lift_stack n k π)
+  | Case_brs ci pred c brctx brs1 brs2 π =>
+      let k' := #|stack_context π| + k in
+      let brs1' := map_branches_k (lift n) k' brs1 in
+      let brs2' := map_branches_k (lift n) k' brs2 in
+      let pred' := map_predicate id (lift n k') (lift n (#|pred.(pcontext)| + k')) pred in
+      Case_brs ci pred' (lift n k' c) (lift_context n k' brctx) brs1' brs2' (lift_stack n k π)
   | Proj p π =>
       Proj p (lift_stack n k π)
   | Prod_l na B π =>
@@ -2036,6 +524,44 @@ Proof.
   rewrite mapi_length. reflexivity.
 Qed.
 
+Lemma map_decl_name_fold_context f ctx : 
+  map decl_name (fold_context f ctx) = map decl_name ctx.
+Proof.
+  now rewrite fold_context_alt map_mapi /= mapi_cst_map.
+Qed.
+
+Lemma forget_types_fold_context f ctx : 
+  forget_types (fold_context f ctx) = forget_types ctx.
+Proof.
+  now rewrite /forget_types map_decl_name_fold_context.
+Qed.
+
+Lemma forget_types_length ctx :
+  #|forget_types ctx| = #|ctx|.
+Proof.
+  now rewrite /forget_types map_length.
+Qed.
+
+Definition lendb := 
+  (rename_context_length,
+   idsn_length,
+   cofix_subst_length,
+   fix_subst_length,
+   fix_context_length,
+   subst_instance_context_length,
+   inds_length,
+   forget_types_length,
+   extended_subst_length,
+   expand_lets_ctx_length,
+   expand_lets_k_ctx_length,
+   lift_context_length,
+   @map_InP_length,
+   context_assumptions_lift_context,
+   context_assumptions_subst_context,
+   context_assumptions_subst_instance_context,
+   context_assumptions_app,
+   app_context_length).
+
 Lemma lift_zipc :
   forall n k t π,
     let k' := #|stack_context π| + k in
@@ -2069,7 +595,13 @@ Proof.
     rewrite !app_length. cbn. rewrite !map_length.
     f_equal. f_equal. lia.
   - simpl. rewrite IHπ. cbn. f_equal. f_equal.
-    rewrite map_app. cbn. reflexivity.
+    now rewrite /map_predicate /= map_app /= /id.
+  - simpl. rewrite IHπ; cbn. f_equal. f_equal.
+    rewrite /map_predicate /=.
+    now rewrite forget_types_fold_context !lendb Nat.add_assoc.
+  - simpl. rewrite IHπ; cbn. f_equal. f_equal.
+    rewrite map_app /=. f_equal. f_equal.
+    now rewrite /map_branch /= forget_types_fold_context !lendb.
 Qed.
 
 Lemma weakening_cumul `{CF:checker_flags} Σ Γ Γ' Γ'' M N :
@@ -2085,318 +617,9 @@ Proof.
     econstructor 3; eauto.
 Qed.
 
-Lemma destArity_it_mkProd_or_LetIn ctx ctx' t :
-  destArity ctx (it_mkProd_or_LetIn ctx' t) =
-  destArity (ctx ,,, ctx') t.
-Proof.
-  induction ctx' in ctx, t |- *; simpl; auto.
-  rewrite IHctx'. destruct a as [na [b|] ty]; reflexivity.
-Qed.
-
-Lemma lift_build_case_predicate_type ind mdecl idecl u params ps n k :
-  closed_ctx (subst_instance_context u (ind_params mdecl)) ->
-  build_case_predicate_type ind mdecl
-    (map_one_inductive_body (context_assumptions mdecl.(ind_params))
-            (length (arities_context (ind_bodies mdecl))) (fun k' => lift n (k' + k))
-            (inductive_ind ind) idecl)
-    (map (lift n k) params) u ps
-  = option_map (lift n k) (build_case_predicate_type ind mdecl idecl params u ps).
-Proof.
-  intros closedpars. unfold build_case_predicate_type.
-  rewrite -> ind_type_map. simpl.
-  epose proof (lift_instantiate_params n k _ params (subst_instance_constr u (ind_type idecl))) as H.
-  rewrite <- lift_subst_instance_constr.
-  erewrite <- H; trivial. clear H.
-  case_eq (instantiate_params (subst_instance_context u (ind_params mdecl)) params (subst_instance_constr u (ind_type idecl))) ; cbnr.
-  intros ity eq.
-  pose proof (lift_destArity [] ity n k) as H; cbn in H. rewrite H; clear H.
-  destruct destArity as [[ctx s] | ]; [|reflexivity]. simpl. f_equal.
-  rewrite lift_it_mkProd_or_LetIn; cbn. unf_term. f_equal. f_equal.
-  - destruct idecl; reflexivity.
-  - rewrite lift_mkApps; cbn; f_equal. rewrite map_app. f_equal.
-    + rewrite !map_map lift_context_length; apply map_ext. clear.
-      intro. now rewrite -> permute_lift by lia.
-    + now rewrite -> to_extended_list_lift, <- to_extended_list_map_lift.
-Qed.
-
-Lemma lift_build_branches_type ind mdecl idecl u p params n k :
-  closed_ctx (subst_instance_context u (ind_params mdecl)) ->
-  build_branches_type ind mdecl
-         (map_one_inductive_body (context_assumptions mdecl.(ind_params))
-            #|arities_context (ind_bodies mdecl)| (fun k' => lift n (k' + k))
-            (inductive_ind ind) idecl)
-         (map (lift n k) params) u (lift n k p)
-  = map (option_map (on_snd (lift n k)))
-        (build_branches_type ind mdecl idecl params u p).
-Proof.
-  intros closedpars. unfold build_branches_type.
-  rewrite -> ind_ctors_map.
-  rewrite -> mapi_map, map_mapi. eapply mapi_ext. intros i x.
-  destruct x as [[id t] arity]. simpl.
-  rewrite <- lift_subst_instance_constr.
-  rewrite subst0_inds_lift.
-  rewrite <- lift_instantiate_params ; trivial.
-  match goal with
-  | |- context [ option_map _ (instantiate_params ?x ?y ?z) ] =>
-    destruct (instantiate_params x y z) eqn:Heqip; cbnr
-  end.
-  epose proof (lift_decompose_prod_assum t0 n k).
-  destruct (decompose_prod_assum [] t0).
-  rewrite <- H.
-  destruct (decompose_app t1) as [fn arg] eqn:?.
-  rewrite (decompose_app_lift _ _ _ fn arg); auto. simpl.
-  destruct (chop _ arg) eqn:Heqchop.
-  eapply chop_map in Heqchop.
-  rewrite -> Heqchop. clear Heqchop.
-  unfold on_snd. simpl. f_equal.
-  rewrite -> lift_it_mkProd_or_LetIn, !lift_mkApps, map_app; simpl.
-  rewrite -> !lift_mkApps, !map_app, lift_context_length.
-  rewrite -> permute_lift by lia. arith_congr.
-  now rewrite -> to_extended_list_lift, <- to_extended_list_map_lift.
-Qed.
-
 Lemma destInd_lift n k t : destInd (lift n k t) = destInd t.
 Proof.
   destruct t; simpl; try congruence.
-Qed.
-
-Lemma weakening_check_one_fix (Γ' Γ'' : context) mfix :
-  map
-       (fun x : def term =>
-        check_one_fix (map_def (lift #|Γ''| #|Γ'|) (lift #|Γ''| (#|mfix| + #|Γ'|)) x)) mfix =
-  map check_one_fix mfix.
-Proof.
-  apply map_ext. move=> [na ty def rarg] /=.
-  rewrite decompose_prod_assum_ctx.
-  destruct (decompose_prod_assum _ ty) eqn:decomp.
-  rewrite decompose_prod_assum_ctx in decomp.
-  rewrite -lift_decompose_prod_assum.
-  destruct (decompose_prod_assum [] ty) eqn:decty.
-  noconf decomp. rewrite !app_context_nil_l (smash_context_lift []).
-  destruct (nth_error_spec (List.rev (smash_context [] c0)) rarg);
-  autorewrite with len in *; simpl in *.
-  - rewrite nth_error_rev_inv; autorewrite with len; simpl; auto.
-    rewrite nth_error_lift_context_eq.
-    simpl.
-    rewrite nth_error_rev_inv in e; autorewrite with len; auto.
-    autorewrite with len in e. simpl in e. rewrite e. simpl.
-    destruct (decompose_app (decl_type x)) eqn:Happ.
-    erewrite decompose_app_lift; eauto.
-    rewrite destInd_lift. reflexivity.
-  - erewrite (proj2 (nth_error_None _ _)); auto.
-    autorewrite with len. simpl; lia.
-Qed.
-
-Lemma weakening_check_one_cofix (Γ' Γ'' : context) mfix :
-  map
-       (fun x : def term =>
-        check_one_cofix (map_def (lift #|Γ''| #|Γ'|) (lift #|Γ''| (#|mfix| + #|Γ'|)) x)) mfix =
-  map check_one_cofix mfix.
-Proof.
-  apply map_ext. move=> [na ty def rarg] /=.
-  rewrite decompose_prod_assum_ctx.
-  destruct (decompose_prod_assum _ ty) eqn:decomp.
-  rewrite decompose_prod_assum_ctx in decomp.
-  rewrite -lift_decompose_prod_assum.
-  destruct (decompose_prod_assum [] ty) eqn:decty.
-  noconf decomp.
-  destruct (decompose_app t) eqn:Happ.
-  erewrite decompose_app_lift; eauto.
-  rewrite destInd_lift. reflexivity.
-Qed.
-
-Lemma weakening_typing_prop {cf:checker_flags} : env_prop (fun Σ Γ0 t T =>
-  forall Γ Γ' Γ'' : context,
-  wf_local Σ (Γ ,,, Γ'') ->
-  Γ0 = Γ ,,, Γ' ->
-  Σ;;; Γ ,,, Γ'' ,,, lift_context #|Γ''| 0 Γ' |- lift #|Γ''| #|Γ'| t : lift #|Γ''| #|Γ'| T)
-  (fun Σ Γ0 _  =>
-  forall Γ Γ' Γ'' : context,
-  Γ0 = Γ ,,, Γ' ->
-  wf_local Σ (Γ ,,, Γ'') ->
-  wf_local Σ (Γ ,,, Γ'' ,,, lift_context #|Γ''| 0 Γ')).
-Proof.
-  apply typing_ind_env;
-    intros Σ wfΣ Γ0; !!intros; subst Γ0; simpl in *; try solve [econstructor; eauto];
-        try specialize (forall_Γ  _ _ _ eq_refl wf).
-
-  - induction Γ'; simpl; auto.
-    depelim X; rewrite lift_context_snoc; simpl; constructor.
-    + eapply IHΓ'; eauto.
-    + red. exists (tu.π1). simpl.
-      rewrite Nat.add_0_r. apply t0; auto.
-    + eapply IHΓ'; eauto.
-    + red. exists (tu.π1). simpl.
-      rewrite Nat.add_0_r. apply t1; auto.
-    + simpl. rewrite Nat.add_0_r. apply t0; auto.
-
-  - elim (leb_spec_Set); intros Hn.
-    + rewrite -> simpl_lift; try lia. rewrite -> Nat.add_succ_r.
-      constructor. 1: auto.
-      now rewrite <- (weaken_nth_error_ge Hn).
-    + assert (forall t, lift0 (S n) (lift #|Γ''| (#|Γ'| - S n) t) = lift #|Γ''| #|Γ'| (lift0 (S n) t)).
-      * intros.
-        assert (H:#|Γ'| = S n + (#|Γ'| - S n)) by easy.
-        rewrite -> H at 2.
-        rewrite permute_lift; easy.
-      * rewrite <- H.
-        rewrite -> map_decl_type. constructor; auto.
-        now rewrite -> (weaken_nth_error_lt Hn), heq_nth_error.
-
-  - econstructor; auto.
-    specialize (IHb Γ (Γ' ,, vass n t) Γ'' wf eq_refl).
-    rewrite -> lift_context_snoc, plus_0_r in IHb.
-    eapply IHb.
-
-  - econstructor; auto.
-    simpl.
-    specialize (IHb Γ (Γ' ,, vass n t) Γ'' wf eq_refl).
-    rewrite -> lift_context_snoc, plus_0_r in IHb.
-    eapply IHb.
-
-  - econstructor; auto.
-    specialize (IHb Γ Γ' Γ'' wf eq_refl). simpl.
-    specialize (IHb' Γ (Γ' ,, vdef n b b_ty) Γ'' wf eq_refl).
-    rewrite -> lift_context_snoc, plus_0_r in IHb'.
-    apply IHb'.
-
-  - eapply refine_type. 1: econstructor; auto.
-    now rewrite -> distr_lift_subst10.
-
-  - autorewrite with lift.
-    rewrite -> map_cst_type. constructor; auto.
-    erewrite <- lift_declared_constant; eauto.
-
-  - autorewrite with lift.
-    erewrite <- (ind_type_map (fun k' => lift #|Γ''| (k' + #|Γ'|))).
-    pose proof isdecl as isdecl'.
-    destruct isdecl. intuition auto.
-    eapply lift_declared_inductive in 2: isdecl'. auto.
-    rewrite -> isdecl'.
-    econstructor; try red; intuition eauto.
-
-  - rewrite (lift_declared_constructor _ (ind, i) u mdecl idecl cdecl _ _ wfΣ isdecl).
-    econstructor; eauto.
-
-  - rewrite -> lift_mkApps, map_app, map_skipn.
-    specialize (IHc _ _ _ wf eq_refl).
-    specialize (IHp _ _ _ wf eq_refl).
-    assert (Hclos: closed_ctx (subst_instance_context u (ind_params mdecl))). {
-      destruct isdecl as [Hmdecl Hidecl].
-      eapply on_declared_minductive in Hmdecl; eauto.
-      eapply onParams in Hmdecl.
-      rewrite closedn_subst_instance_context.
-      eapply closed_wf_local in Hmdecl; eauto. }
-    simpl. econstructor.
-    8:{ cbn. rewrite -> firstn_map.
-        erewrite lift_build_branches_type; tea.
-        rewrite map_option_out_map_option_map.
-        subst params. erewrite heq_map_option_out. reflexivity. }
-    all: eauto.
-    -- erewrite -> lift_declared_inductive; eauto.
-    -- simpl. erewrite firstn_map, lift_build_case_predicate_type; tea.
-       subst params. erewrite heq_build_case_predicate_type; reflexivity.
-    -- destruct idecl; simpl in *; auto.
-    -- now rewrite -> !lift_mkApps in IHc.
-    -- solve_all.
-      destruct b0 as [s [Hs IH]]; eauto.
-
-  - simpl.
-    erewrite (distr_lift_subst_rec _ _ _ 0 #|Γ'|).
-    simpl. rewrite -> map_rev.
-    subst ty.
-    rewrite -> List.rev_length, lift_subst_instance_constr.
-    replace (lift #|Γ''| (S (#|args| + #|Γ'|)) (snd pdecl))
-      with (snd (on_snd (lift #|Γ''| (S (#|args| + #|Γ'|))) pdecl)) by now destruct pdecl.
-    econstructor.
-    + red. split.
-      * apply (proj1 isdecl).
-      * split.
-        -- rewrite -> (proj1 (proj2 isdecl)). f_equal.
-           rewrite -> heq_length.
-           symmetry. eapply lift_declared_projection; eauto.
-        -- apply (proj2 (proj2 isdecl)).
-    + specialize (IHc _ _ _ wf eq_refl).
-      rewrite -> lift_mkApps in *. eapply IHc.
-    + now rewrite -> map_length.
-
-  - rewrite -> (map_dtype _ (lift #|Γ''| (#|mfix| + #|Γ'|))).
-    eapply type_Fix; auto.
-    * eapply fix_guard_lift ; eauto.
-    * rewrite -> nth_error_map, heq_nth_error. reflexivity.
-    * eapply All_map.
-      eapply (All_impl X0); simpl.
-      intros x [s [Hs Hs']]; exists s.
-      now specialize (Hs' _ _ _ wf eq_refl).
-    * eapply All_map.
-      eapply (All_impl X1); simpl.
-      intros x [Hb IH].
-      rewrite lift_fix_context.
-      specialize (IH Γ (Γ' ,,,  (fix_context mfix)) Γ'' wf).
-      rewrite app_context_assoc in IH. specialize (IH eq_refl).
-      rewrite lift_context_app Nat.add_0_r app_context_assoc in IH.
-      rewrite app_context_length fix_context_length in IH.
-      rewrite lift_context_length fix_context_length.
-      rewrite permute_lift; try lia. now rewrite (Nat.add_comm #|Γ'|).
-    * red; rewrite <-H1. unfold wf_fixpoint.
-      rewrite map_map_compose.
-      now rewrite weakening_check_one_fix.
-
-  - rewrite -> (map_dtype _ (lift #|Γ''| (#|mfix| + #|Γ'|))).
-    eapply type_CoFix; auto.
-    * eapply cofix_guard_lift ; eauto.
-    * rewrite -> nth_error_map, heq_nth_error. reflexivity.
-    * eapply All_map.
-      eapply (All_impl X0); simpl.
-      intros x [s [Hs Hs']]; exists s.
-      now specialize (Hs' _ _ _ wf eq_refl).
-    * eapply All_map.
-      eapply (All_impl X1); simpl.
-      intros x [Hb IH].
-      rewrite lift_fix_context.
-      specialize (IH Γ (Γ' ,,,  (fix_context mfix)) Γ'' wf).
-      rewrite app_context_assoc in IH. specialize (IH eq_refl).
-      rewrite lift_context_app Nat.add_0_r app_context_assoc in IH.
-      rewrite app_context_length fix_context_length in IH.
-      rewrite lift_context_length fix_context_length.
-      rewrite permute_lift; try lia. now rewrite (Nat.add_comm #|Γ'|).
-    * red; rewrite <-H1. unfold wf_cofixpoint.
-      rewrite map_map_compose.
-      now rewrite weakening_check_one_cofix.
-
-  - econstructor; eauto; now eapply weakening_cumul.
-Qed.
-
-Lemma weakening_typing `{cf : checker_flags} Σ Γ Γ' Γ'' (t : term) :
-  wf Σ.1 ->
-  wf_local Σ (Γ ,,, Γ'') ->
-  forall T, Σ ;;; Γ ,,, Γ' |- t : T ->
-       Σ ;;; Γ ,,, Γ'' ,,, lift_context #|Γ''| 0 Γ' |-
-       lift #|Γ''| #|Γ'| t : lift #|Γ''| #|Γ'| T.
-Proof.
-  intros HΣ HΓ'' T H.
-  exact ((weakening_typing_prop Σ HΣ _ t T H).2 _ _ _ HΓ'' eq_refl).
-Qed.
-
-Lemma weakening_wf_local `{cf : checker_flags} Σ Γ Γ' Γ'' :
-  wf Σ.1 ->
-  wf_local Σ (Γ ,,, Γ') ->
-  wf_local Σ (Γ ,,, Γ'') ->
-  wf_local Σ (Γ ,,, Γ'' ,,, lift_context #|Γ''| 0 Γ').
-Proof.
-  intros HΣ HΓΓ' HΓ''.
-  exact (env_prop_wf_local _ _ weakening_typing_prop
-                           Σ HΣ _ HΓΓ' _ _ _ eq_refl HΓ'').
-Qed.
-
-Lemma weakening `{cf : checker_flags} Σ Γ Γ' (t : term) T :
-  wf Σ.1 -> wf_local Σ (Γ ,,, Γ') ->
-  Σ ;;; Γ |- t : T ->
-  Σ ;;; Γ ,,, Γ' |- lift0 #|Γ'| t : lift0 #|Γ'| T.
-Proof.
-  intros HΣ HΓΓ' * H.
-  pose (weakening_typing Σ Γ [] Γ' t).
-  forward t0; eauto.
 Qed.
 
 (** Variant with more freedom on the length to apply it in backward-chainings. *)
@@ -2424,19 +647,17 @@ Proof.
 Qed.
 
 Lemma weaken_ctx {cf:checker_flags} {Σ Γ t T} Δ :
-  wf Σ.1 -> wf_local Σ Δ ->
+  wf Σ.1 -> 
+  wf_local Σ Δ ->
   Σ ;;; Γ |- t : T ->
   Σ ;;; Δ ,,, Γ |- t : T.
 Proof.
   intros wfΣ wfΔ ty.
-  epose proof (weakening_typing Σ [] Γ Δ t wfΣ).
+  epose proof (weakening_typing (Γ := [])).
   rewrite !app_context_nil_l in X.
   forward X by eauto using typing_wf_local.
-  pose proof (typing_wf_local ty).
-  pose proof (closed_wf_local wfΣ (typing_wf_local ty)).
-  specialize (X _ ty).
-  eapply PCUICClosed.typecheck_closed in ty as [_ closed]; auto.
-  move/andb_and: closed => [ct cT].
+  specialize (X ty).
+  eapply PCUICClosed.typecheck_closed in ty as [_ [clΓ [clt clT]%andb_and]]; auto.
   rewrite !lift_closed // in X.
   now rewrite closed_ctx_lift in X.
 Qed.
@@ -2451,9 +672,9 @@ Proof.
 Qed.
 
 Corollary All_mfix_wf {cf:checker_flags} Σ Γ mfix :
- wf Σ.1 -> wf_local Σ Γ ->
- All (fun d : def term => isType Σ Γ (dtype d)) mfix ->
- wf_local Σ (Γ ,,, fix_context mfix).
+  wf Σ.1 -> wf_local Σ Γ ->
+  All (fun d : def term => isType Σ Γ (dtype d)) mfix ->
+  wf_local Σ (Γ ,,, fix_context mfix).
 Proof.
   move=> wfΣ wf a; move: wf.
   change (fix_context mfix) with (fix_context_gen #|@nil context_decl| mfix).
@@ -2492,5 +713,6 @@ Proof.
   { rewrite firstn_length_le; auto with arith. }
   destruct wfty as [u Hu]. exists u.
   rewrite {3}H.
-  unshelve eapply (weakening_typing Σ (skipn n Γ) [] (firstn n Γ) ty _ _ (tSort u)); eauto with wf.
+  eapply (weakening_typing (Γ := skipn n Γ) (Γ' := []) (Γ'' := firstn n Γ) (T := tSort u)); 
+    eauto with wf.
 Qed.
